Cleanup in progress

Eval.v
@@ -1,310 +1,316 @@
 (* Celsius project *)
-(* Clément Blaudeau *)
+(* Clément Blaudeau - LAMP@EPFL 2021 *)
+(** This file defines the evaluator of the language and some general results *)
 
-(** Definition of the evaluator of the Celsius Model *)
 From Celsius Require Export Trees Tactics.
 Require Import ssreflect ssrbool.
 Require Import Celsius.strongInduction.
 Require Import List.
+Require Import Psatz.
 Import ListNotations.
 Open Scope nat_scope.
 
+(** The classtable is assumed generaly accessible *)
+Parameter ct: ClassTable.
 
-(** * Evaluator Module  *)
-Module Evaluator.
-  (** The classtable is assumed generaly accessible *)
-  Parameter ct: ClassTable.
+(** ** Helper functions *)
 
-  (** ** Helper functions *)
+(** Update store with new value in local env : adds a new field to an existing object *)
+Definition assign_new (obj: Value) (v: Value) (σ: Store) : option Store :=
+  match (getObj σ obj) with
+  | Some (C, fields) => Some ([ obj ↦ (C, fields++[v])] σ)
+  | None => None (* ? *)
+  end.
 
-  (** Update store with new value in local env : adds a new field to an existing object *)
-  Definition assign_new (obj: Value) (v: Value) (σ: Store) : option Store :=
-    match (getObj σ obj) with
-    | Some (C, fields) => Some ([ obj ↦ (C, fields++[v])] σ)
-    | None => None (* ? *)
-    end.
+(** Update store with update in local env : update an already-existing field of an existing object*)
+Definition assign (obj: Value) (f: Var) (v: Value) (σ: Store) : Store :=
+  match (getObj σ obj) with
+  | Some (C, fields) => ([ obj ↦ (C, [f ↦ v]fields)] σ)
+  | None => σ (* ? *)
+  end.
 
-  (** Update store with update in local env : update an already-existing field of an existing object*)
-  Definition assign (obj: Value) (f: Var) (v: Value) (σ: Store) : Store :=
-    match (getObj σ obj) with
-    | Some (C, fields) => ([ obj ↦ (C, [f ↦ v]fields)] σ)
-    | None => σ (* ? *)
-    end.
+(** Update store with new values : update already existing fields of an existing object*)
+Definition assign_list (v0: Value) (x: list Var) (v: list Value) (σ: Store) : Store :=
+  match (getObj σ v0) with
+  | Some (C, fields) => [v0 ↦ (C, [x ⟼ v]fields)] σ
+  | None => σ
+  end.
 
-  (** Update store with new values : update already existing fields of an existing object*)
-  Definition assign_list (v0: Value) (x: list Var) (v: list Value) (σ: Store) : Store :=
-    match (getObj σ v0) with
-    | Some (C, fields) => [v0 ↦ (C, [x ⟼ v]fields)] σ
-    | None => σ
-    end.
+(** ** Evaluation results *)
 
-  (** ** Main small-step evaluator *)
+(* Evaluation result *)
+Inductive result : Type :=
+| Timeout
+| Error
+| Success : Value -> Store -> result.
 
-  (* Evaluation result *)
-  Inductive Result : Type :=
-  | Timeout
-  | Error
-  | Success : Value -> Store -> Result
-  .
-  Inductive Result_l : Type :=
-  | Timeout_l
-  | Error_l
-  | Success_l : (list Value) -> Store -> Result_l
-  .
+Inductive result_l : Type :=
+| Timeout_l
+| Error_l
+| Success_l : (list Value) -> Store -> result_l.
 
 
-  Reserved Notation "'⟦' e '⟧' '(' σ ',' ρ ',' v ')(' k ')'"   (at level 80).
-  Reserved Notation "'⟦_' e '_⟧' '(' σ ',' ρ ',' v ')(' k ')'" (at level 80).
-  Fixpoint eval (e: Expr) (σ: Store) (ρ: Env) (v: Value) (k: nat) : Result :=
-    match k with
-    | 0 => Timeout
-    | S n => match e with
-            (**r e = x *)
-            (**r Var: simple lookup of the store *)
-            | var x => (
-                match (getVal ρ x) with
-                | Some v => (Success v σ)
-                | _ => Error
-                end )
+(** ** Big step evaluator (with fuel) *)
+(** We define the [eval] function along with its notations *)
 
-            (* e = this *)
-            (* This: returns current value *)
-            | this => (Success v σ)
+Reserved Notation "'⟦' e '⟧' '(' σ ',' ρ ',' v ')(' k ')'"   (at level 80).
+Reserved Notation "'⟦_' e '_⟧' '(' σ ',' ρ ',' v ')(' k ')'" (at level 80).
+Fixpoint eval e σ ρ v k :=
+  match k with
+  | 0 => Timeout
+  | S n => match e with
+          (** Var: simple lookup of the store *)
+          | var x => (**r [e = x] *)
+            (match (getVal ρ x) with
+             | Some v => (Success v σ)
+             | _ => Error
+             end )
 
-            (* e = e0.x *)
-            (* Field access: compute object value and access field *)
-            | fld e0 x => (
-                match (⟦e0⟧(σ, ρ, v)(n)) with
-                | Success v0 σ1 =>
-                  match (getObj σ1 v0) with
-                  | Some (c, f) =>
-                    match (getVal f x) with
-                    | Some v1 => Success v1 σ1
-                    | _ => Error end
+          (** This: returns current value *)
+          | this => (Success v σ) (**r [e = this] *)
+
+          (** Field access: compute object value and access field *)
+          | fld e0 x => (**r [e = e0.x] *)
+            ( match (⟦e0⟧(σ, ρ, v)(n)) with
+              | Success v0 σ1 =>
+                match (getObj σ1 v0) with
+                | Some (c, f) =>
+                  match (getVal f x) with
+                  | Some v1 => Success v1 σ1
                   | _ => Error end
-                | _ => Error end )
+                | _ => Error end
+              | _ => Error end )
 
-            (* e = e.m(el) *)
-            (* Method call : compute object value, compute arguments and do the call*)
-            | mtd e0 m el => (
-                match (⟦e0⟧(σ, ρ, v)(n)) with
-                | Success v0 σ1 => (
-                    match (getObj σ1 v0) with
-                    | Some (C, _) => (
-                        match (ct C)  with
-                        | Some (class _  _ methods) => (
-                            match methods m with
-                            | Some (method μ x _ e1) => (
-                                match (⟦_ el _⟧(σ1, ρ, v)(n)) with
-                                | Success_l args_val σ2 =>
-                                  let ρ1 := args_val in ⟦e1⟧(σ2, ρ1, v0)(n)
-                                | _ => Error end)
-                            | _ => Error end)
-                        | _ => Error end)
-                    | _ => Error end)
-                | _ => Error end)
+          (** Method call : compute object value, compute arguments and do the call*)
+          | mtd e0 m el => (**r [e = e0.m(el)] *)
+            (match (⟦e0⟧(σ, ρ, v)(n)) with
+             | Success v0 σ1 => (
+                 match (getObj σ1 v0) with
+                 | Some (C, _) => (
+                     match (ct C)  with
+                     | Some (class _  _ methods) => (
+                         match methods m with
+                         | Some (method μ x _ e1) => (
+                             match (⟦_ el _⟧(σ1, ρ, v)(n)) with
+                             | Success_l args_val σ2 =>
+                               let ρ1 := args_val in ⟦e1⟧(σ2, ρ1, v0)(n)
+                             | _ => Error end)
+                         | _ => Error end)
+                     | _ => Error end)
+                 | _ => Error end)
+             | _ => Error end)
 
-            (* e = new C(args) *)
-            (* New class *)
-            | new C args => (
-                match (⟦_ args _⟧(σ, ρ, v)(n)) with
-                | Success_l args_val σ1 => (
-                    let I := (length σ1) in (* Fresh location for new object *)
-                    let ρ_init := args_val in (* Local env during initialisation *)
-                    let σ2 := σ1 ++ [(C, ∅)] in (* New object with empty local env *)
-                      match (init I ρ_init C σ2 n) with
-                      | Some σ3 => (Success I σ3) (* Returns new object and updated store *)
-                      | None => Error end )
-                | _ => Error end) (* Invalid args *)
+          (** New class *)
+          | new C args => (**r [e = new C(args)] *)
+            (match (⟦_ args _⟧(σ, ρ, v)(n)) with
+             | Success_l args_val σ1 => (
+                 let I := (length σ1) in (* Fresh location for new object *)
+                 let ρ_init := args_val in (* Local env during initialisation *)
+                 let σ2 := σ1 ++ [(C, ∅)] in (* New object with empty local env *)
+                 match (init I ρ_init C σ2 n) with
+                 | Some σ3 => (Success I σ3) (* Returns new object and updated store *)
+                 | None => Error end )
+             | _ => Error end) (* Invalid args *)
 
-            (* e = (e1.x ← e2 ; e') *)
-            (* Field assignement *)
-            | asgn e1 x e2 e' => (
-                match (⟦e1⟧(σ, ρ, v)(n)) with
-                | Success v1 σ1 => match (⟦e2⟧(σ1, ρ, v)(n)) with
-                                  | Success v2 σ2 => (
-                                      let σ3 := (assign v1 x v2 σ2) in
-                                      ⟦e'⟧(σ3, ρ, v)(n))
-                                  | _ => Error end
-                | _ => Error end )
-            end
-    end
-  where "'⟦' e '⟧' '(' σ ',' ρ ',' v ')(' k ')'"  := (eval e σ ρ v k)
-  with eval_list (e_l: list Expr) (σ: Store) (ρ: Env) (v: Value) (k: nat): Result_l :=
-         match k with
-         | 0 => Timeout_l
-         | S n => fold_left (eval_list_aux ρ v n) e_l (Success_l [] σ) end
-  where  "'⟦_' e '_⟧' '(' σ ',' ρ ',' v ')(' k ')'" := (eval_list e σ ρ v k)
-  with eval_list_aux (ρ: Env) (v: Value) (k: nat) acc (e: Expr) :=
-         match k with
-         | 0 => Timeout_l
-         | S n => match acc with
-                 | Success_l vs σ1 => match (⟦e⟧(σ1, ρ, v)(n)) with
-                                        | Success v σ2 => Success_l (v::vs) σ2
-                                        | Timeout => Timeout_l
-                                        | Error => Error_l
-                                     end
-                 | z => z end end
-  with init (I : Var) (args_values: list Var) (C: ClN) (σ: Store) (k :nat) : option Store :=
-         match k with | 0 => None | S n =>
-           match (ct C) with
-           | Some (class x F M) => (fold_left (init_field args_values I n) F (Some σ))
-           | None => None
-           end
-         end
-  with init_field (args_values: list Var) (this: Var) (k: nat) (σ_opt: option Store)  (f: Field): option Store :=
-         match k with
-         | 0 => None
-         | S n =>
-           match σ_opt with
-           | None => None
-           | Some σ => ( match f with
-                        | field t e => (
-                            match (⟦e⟧(σ, args_values, this)(n)) with
-                            | Success v1 σ1 => (assign_new this v1 σ1)
-                            | _ => None
-                            end) end) end end.
+          (** Field assignement *)
+          | asgn e1 x e2 e' => (**r [e = (e1.x ← e2 ; e')] *)
+            (match (⟦e1⟧(σ, ρ, v)(n)) with
+             | Success v1 σ1 => match (⟦e2⟧(σ1, ρ, v)(n)) with
+                               | Success v2 σ2 => (
+                                   let σ3 := (assign v1 x v2 σ2) in
+                                   ⟦e'⟧(σ3, ρ, v)(n))
+                               | _ => Error end
+             | _ => Error end )
+          end
+  end
+where "'⟦' e '⟧' '(' σ ',' ρ ',' v ')(' k ')'"  := (eval e σ ρ v k)
+(** Evaluation of a list of expressions (fold) *)
+with eval_list (e_l: list Expr) (σ: Store) (ρ: Env) (v: Value) (k: nat) :=
+       match k with
+       | 0 => Timeout_l
+       | S n => fold_left (eval_list_aux ρ v n) e_l (Success_l [] σ) end
+where  "'⟦_' e '_⟧' '(' σ ',' ρ ',' v ')(' k ')'" := (eval_list e σ ρ v k)
+with eval_list_aux (ρ: Env) (v: Value) (k: nat) acc (e: Expr) :=
+       match k with
+       | 0 => Timeout_l
+       | S n => match acc with
+               | Success_l vs σ1 => match (⟦e⟧(σ1, ρ, v)(n)) with
+                                   | Success v σ2 => Success_l (v::vs) σ2
+                                   | Timeout => Timeout_l
+                                   | Error => Error_l
+                                   end
+               | z => z end end
+(** Initialization of a list of fields using (fold) *)
+with init (I : Var) (args_values: list Var) (C: ClN) (σ: Store) (k :nat) : option Store :=
+       match k with | 0 => None | S n =>
+                                 match (ct C) with
+                                 | Some (class x F M) => (fold_left (init_field args_values I n) F (Some σ))
+                                 | None => None
+                                 end
+       end
+with init_field (args_values: list Var) (this: Var) (k: nat) (σ_opt: option Store)  (f: Field): option Store :=
+       match k with
+       | 0 => None
+       | S n =>
+         match σ_opt with
+         | None => None
+         | Some σ => ( match f with
+                      | field t e => (
+                          match (⟦e⟧(σ, args_values, this)(n)) with
+                          | Success v1 σ1 => (assign_new this v1 σ1)
+                          | _ => None
+                          end) end) end end.
 
+(** A usefull lemma to show that folds on computations that got stuck (error or timeout) will stay stuck *)
+Lemma foldLeft_constant : forall (A B: Type) (l: list B) (res: A) (f : A -> B -> A),
+    (forall (y:B), f res y = res) -> fold_left f l res = res.
+Proof.
+  intros.
+  induction l => //.
+  simpl. rewrite H. apply IHl.
+Qed.
 
-  Lemma foldLeft_constant : forall (A B: Type) (l: list B) (res: A) (f : A -> B -> A),
-      (forall (y:B), f res y = res) -> fold_left f l res = res.
-    intros.
-    induction l => //.
-    simpl. rewrite H. apply IHl.
-  Qed.
+(** Associated ltac tactics : *)
+Ltac destruct_eval :=
+  match goal with
+  | H: context[⟦ ?e ⟧ (?σ, ?ρ, ?ψ )( ?k)] |- _ =>
+    let fresh_H := fresh H in
+    destruct (⟦ e ⟧ (σ, ρ, ψ )( k)) eqn:fresh_H ;
+    try solve [rewrite foldLeft_constant in H => //]
+  end.
 
-  Ltac destruct_eval :=
-    match goal with
-    | H: context[⟦ ?e ⟧ (?σ, ?ρ, ?ψ )( ?k)] |- _ =>
-      let fresh_H := fresh H in
-      destruct (⟦ e ⟧ (σ, ρ, ψ )( k)) eqn:fresh_H ;
-      try solve [rewrite foldLeft_constant in H => //]
-    end.
+Ltac destruct_eval_with_name fresh_H :=
+  match goal with
+  | H: context[⟦ ?e ⟧ (?σ, ?ρ, ?ψ )( ?k)] |- _ =>
+    destruct (⟦ e ⟧ (σ, ρ, ψ )( k)) eqn:fresh_H ;
+    try solve [rewrite foldLeft_constant in H => //]
+  end.
 
-
-  Definition Reflexive (P: Store -> Store -> Prop) : Prop := (forall σ, P σ σ).
-  Definition Transitive (P: Store -> Store -> Prop)  : Prop := forall (σ1 σ2 σ3: Store), P σ1 σ2 ->  P σ2 σ3 ->  P σ1 σ3.
-  Definition Assignment (P: Store -> Store -> Prop)  : Prop := forall σ σ' l C ω ω',
-          getObj σ l = Some (C, ω) ->
-          length ω <= length ω' ->
-          σ' = [l ↦ (C, ω')]σ -> P σ σ'.
-  Definition Freshness (P: Store -> Store -> Prop) : Prop := forall s c ω, P s (s ++ [(c, ω)]).
-
-
-  Definition EvalMaintained (P: Store -> Store -> Prop)  k : Prop := forall e σ σ' ρ v v',  ⟦e⟧(σ, ρ, v)(k) = (Success v' σ') -> (P σ σ') .
-
-  Definition InitMaintained (P: Store -> Store -> Prop) (n:nat) : Prop :=
-    (forall (k: nat), (k < n) -> EvalMaintained P k) ->
-    (forall (k: nat), (k < n) ->
-               forall (l0: list Var) (s σ': Store) (c: ClN),
-                 init (length s) l0 c (s ++ [(c, [])]) k = Some σ' -> P s σ').
-
-
-
-
-  Lemma eval_list_prop : forall (P: Store -> Store -> Prop) n,
-      Reflexive P -> Transitive P -> (forall k, (k < n) -> EvalMaintained P k) ->
-      (forall k, (k < n) -> forall l σ σ' ρ v v_list,  ⟦_ l _⟧(σ, ρ, v)(k) = (Success_l v_list σ') -> (P σ σ')).
-    intros P n H_refl H_trans H_strong.
-    destruct k; simpl; try discriminate.
-    assert (forall l σ σ' ρ v v_list1 v_list2,
-               (k < n) ->
-               fold_left (eval_list_aux ρ v k) l (Success_l v_list1 σ) = Success_l v_list2 σ' ->
-               P σ σ');
-      eauto using PeanoNat.Nat.lt_succ_l. {
-      induction l as [| e l]; simpl; intros.
-      + invert_constructor_equalities; eauto.
-      + destruct k; simpl in H0. rewrite foldLeft_constant in H0 => //.
-        move /(_ _ _ _ _ _ _ H):IHl => IHl.
-        move /(_ _ (PeanoNat.Nat.lt_succ_l k n H)):H_strong => H_strong.
-        destruct_eval ; eauto.
-    }
-  Qed.
-
-  Lemma freshnessInitMaintained : forall (P: Store -> Store -> Prop) n,
-      Reflexive P -> Transitive P -> Assignment P -> Freshness P -> InitMaintained P n.
-  Proof.
-    intros P n H_refl H_trans H_asgn H_fresh H_strong.
-    assert ( forall k : nat,
-               k < n ->
-               forall (l0 : list Var) (σ σ' : Store) (c : ClN) I , init I l0 c σ k = Some σ' -> P σ σ');
-      eauto.
-    {
-      destruct k; simpl; try discriminate.
-      intros Hn; intros.
-      repeat destruct_match; try discriminate. clear matched0. clear matched.
-      generalize dependent σ. generalize dependent σ'.
-      induction fields as [| [x e] fields]; simpl; intros.
-      + invert_constructor_equalities; eauto.
-      + destruct k; simpl in H. rewrite foldLeft_constant in H => //.
-        destruct_eval; eauto.
-        unfold assign_new in H.
-        repeat destruct_match; try solve [rewrite foldLeft_constant in H => //].
-        subst.
-        move /(_ _ _ H):IHfields => IHfields.
-        apply PeanoNat.Nat.lt_succ_l in Hn.
-        apply PeanoNat.Nat.lt_succ_l in Hn.
-        move /(_ k Hn _ _ _ _ _ _ H0):H_strong => H_strong.
-        apply (H_trans _ _ _ H_strong).
-        apply (H_trans _  [I ↦ (c1, e0 ++ [v])] (s)  _ ) => //.
-        apply (H_asgn _ _ _ _ _ (e0 ++ [v])  matched); eauto using app_length.
-        rewrite app_length.
-        rewrite PeanoNat.Nat.add_1_r. eauto.
-    }
-  Qed.
-
-    Lemma eval_prop : forall (P: Store -> Store -> Prop),
-        Reflexive P -> Transitive P ->  Assignment P -> (forall n, InitMaintained P n) -> forall n, EvalMaintained P n.
-      intros P H_refl H_trans  H_asgn H_init.
-      apply strong_induction.
-      unfold EvalMaintained.
-      intros n H_strong.
-      move /(_ n H_strong):H_init => H_init.
-    (* To get one step of the evaluator, we destruct n *)
-    destruct n => //. (* n = 0 is discarded automatically *)
-    (* n > 0 - case analysis over e *)
-    move : (PeanoNat.Nat.lt_succ_diag_r n) => Hn.
-    destruct e;
-      (* Trivial cases are handled automatically *)
-      repeat light || invert_constructor_equalities || destruct_match || eauto 3.
-    - (* case e = e0.m(ē) *)
-      apply (iff_sym (PeanoNat.Nat.le_succ_l n (S n))) in Hn.
-      pose proof (eval_list_prop P (S n) H_refl H_trans H_strong n Hn _ _ _ _ _ _ matched3); eauto.
-    - (* case e = new C(l) *)
-      apply (iff_sym (PeanoNat.Nat.le_succ_l n (S n))) in Hn.
-      move /(_ n Hn l0 s σ' c matched0):H_init => H_init.
-      pose proof (eval_list_prop P (S n) H_refl H_trans H_strong n Hn _ _ _ _ _ _ matched).
-      eauto.
-    - (* case e1.v0 = e2 ; e3 *)
-      apply (H_trans σ s σ'); eauto.
-      apply (H_strong n Hn _ _ _ _ _ _ ) in matched0.
-      apply (H_trans s _ _ matched0).
-      apply (H_strong n Hn _ _ _ _ _ _ ) in H.
-      apply (H_trans s0 (assign v1 v v2 s0) σ') => //.
-      unfold assign. repeat destruct_match; eauto using PeanoNat.Nat.eq_le_incl, update_one3.
-    Qed.
-
-    Lemma eval_list_length : forall n el σ σ' ρ ψ l ,
-        ⟦_ el _⟧(σ, ρ, ψ)(n) = Success_l l σ' ->
-        length el = length l.
-    Proof.
-      intros n.
-      destruct n; simpl; try discriminate.
-      assert
-        (forall (l : list Expr) (σ σ' : Store) (ρ : Env) (v : Value) (v_list1 v_list2 : list Value),
-            fold_left (eval_list_aux ρ v n) l (Success_l v_list1 σ) = Success_l v_list2 σ'
-            -> length l + length v_list1 = length v_list2) as H_fold. {
-        induction l as [| e l] ; steps.
-        destruct n; simpl in H. rewrite foldLeft_constant in H => //.
-       destruct_eval.
-        apply IHl in H.
-        simpl in H.
-        rewrite plus_n_Sm => //. }
-      intros.
-      pose proof (H_fold _ _ _ _ _ _ _ H); simpl in H0.
-      rewrite PeanoNat.Nat.add_0_r in H0 => //.
-    Qed.
+(** A simple result on lengths *)
+Lemma EvalListLength :
+  forall n el σ σ' ρ ψ l ,
+    ⟦_ el _⟧(σ, ρ, ψ)(n) = Success_l l σ' ->
+    length el = length l.
+Proof.
+  destruct n; simpl; try discriminate.
+  assert
+    (forall l σ σ' ρ v v_list1 v_list2,
+        fold_left (eval_list_aux ρ v n) l (Success_l v_list1 σ) = Success_l v_list2 σ'
+        -> length l + length v_list1 = length v_list2) as H_fold.
+  {
+    induction l as [| e l] ; steps.
+    destruct n; simpl in H ; [rewrite foldLeft_constant in H => // |].
+    destruct_eval.
+    apply IHl in H.
+    simpl in H.
+    rewrite plus_n_Sm => //.
+  }
+  steps;
+    eapply_anywhere H_fold;
+    rewrite_anywhere PeanoNat.Nat.add_0_r => // .
+Qed.
 
 
+(** ** Results *)
+(** As we will show, if a relationship between stores verifies certain properties, it will be maintained by the evaluator. This is used to prove the partial-monotonicity, compatibility, wellformedness and stackability theorems. The scopability theorem is more involved, as it is a relationship involving both the stores and the locations. *)
 
-  End Evaluator.
+Definition Reflexive (P: Store -> Store -> Prop) : Prop :=
+  forall σ, P σ σ.
+Definition Transitive (P: Store -> Store -> Prop)  : Prop :=
+  forall σ1 σ2 σ3, P σ1 σ2 ->  P σ2 σ3 ->  P σ1 σ3.
+Definition Assignment (P: Store -> Store -> Prop)  : Prop :=
+  forall σ σ' l C ω ω',
+    getObj σ l = Some (C, ω) ->
+    length ω <= length ω' ->
+    σ' = [l ↦ (C, ω')]σ -> P σ σ'.
+Definition Freshness (P: Store -> Store -> Prop) : Prop :=
+  forall s c ω, P s (s ++ [(c, ω)]).
+
+(** A relation maintained by the evaluator. All local-reasoning theorems are about showing that some relations are eval maintained. *)
+Definition EvalMaintained (P: Store -> Store -> Prop)  k : Prop :=
+  forall e σ σ' ρ v v',
+    ⟦e⟧(σ, ρ, v)(k) = Success v' σ' ->
+    P σ σ'.
+
+(** *** Initialization *)
+(** One sub-case is to show relations are maintained through initialization of a new object. This could be the consequence of some general properties, or can be proved ad hoc (like for stackability). It's written for a strong-induction-style proof *)
+Definition InitMaintained (P: Store -> Store -> Prop) (n:nat) : Prop :=
+  (forall k, k < n -> EvalMaintained P k) -> (**r strong induction hypothesis *)
+  forall k,
+    k < n ->
+    forall l0 s σ' c,
+      init (length s) l0 c (s ++ [(c, [])]) k = Some σ' ->
+      P s σ'.
+
+(** Notably, if a relation verifies [Freshness] (and other properties), it will be maintained through initialization. *)
+Lemma FreshnessInitMaintained : forall (P: Store -> Store -> Prop) n,
+    Reflexive P -> Transitive P -> Assignment P -> Freshness P -> InitMaintained P n.
+Proof.
+  intros P n H_refl H_trans H_asgn H_fresh H_strong.
+  assert ( forall k, k < n ->
+                forall l0 σ σ' c I , init I l0 c σ k = Some σ' -> P σ σ'); eauto.
+  destruct k; simpl; try discriminate.
+  intros Hn; intros.
+  repeat destruct_match; try discriminate. clear matched0 matched.
+  move : H. move: σ σ'.
+  induction fields as [| [x e] fields]; [steps | simpl; intros].
+  destruct k; simpl in H; [ rewrite foldLeft_constant in H => // |].
+  destruct_eval_with_name E; eauto.
+  unfold assign_new in *.
+  repeat destruct_match; try solve [rewrite foldLeft_constant in H => //].
+  subst.
+  apply PeanoNat.Nat.lt_succ_l, PeanoNat.Nat.lt_succ_l in Hn.
+  apply H_strong in E => //.
+  eapply (H_trans _ _ _ E).
+  apply (H_trans _  [I ↦ (c1, e0 ++ [v])] (s) ) ; eauto.
+  apply (H_asgn _ _ _ _ _ (e0 ++ [v])  matched); eauto.
+  rewrite app_length; steps; lia.
+Qed.
+
+(** *** Evaluation of lists of expressions *)
+(** Another sub-case is to show that [Reflexive] and [Transitive] eval-maintained relations are also maintained when evaluating a list of expressions *)
+Lemma EvalListMaintained : forall (P: Store -> Store -> Prop) n,
+    Reflexive P ->
+    Transitive P ->
+    (forall k, k < n -> EvalMaintained P k) -> (**r strong induction hypothesis *)
+    forall k,
+      k < n ->
+      forall l σ σ' ρ v v_list,
+        ⟦_ l _⟧(σ, ρ, v)(k) = Success_l v_list σ' ->
+        P σ σ'.
+Proof.
+  intros P n H_refl H_trans H_strong.
+  destruct k; simpl; try discriminate.
+  assert (forall l σ σ' ρ v v_list1 v_list2,
+             (k < n) ->
+             fold_left (eval_list_aux ρ v k) l (Success_l v_list1 σ) = Success_l v_list2 σ' ->
+             P σ σ'); eauto using PeanoNat.Nat.lt_succ_l.
+  induction l as [| e l]; [steps | simpl; intros].
+  destruct k; simpl in *; [rewrite foldLeft_constant in H0 => // |].
+  move /(_ _ _ _ _ _ _ H):IHl => IHl.
+  move /(_ _ (PeanoNat.Nat.lt_succ_l _ _ H)):H_strong => H_strong.
+  destruct_eval ; eauto.
+Qed.
+
+(** *** Main evaluation result *)
+(** We show here that a relation that is [Reflexive], [Transitive], that is maintained through assignment and initialization is maintained by the evaluator. We use strong induction *)
+
+Lemma EvalMaintainedProp : forall (P: Store -> Store -> Prop),
+    Reflexive P -> Transitive P ->  Assignment P -> (forall n, InitMaintained P n) -> forall n, EvalMaintained P n.
+  intros P H_refl H_trans  H_asgn H_init.
+  apply strong_induction.
+  unfold EvalMaintained.
+  intros n H_strong.
+  move /(_ n H_strong):H_init => H_init.
+  (** To get one step of the evaluator, we destruct n *)
+  destruct n => //.
+  move : (PeanoNat.Nat.lt_succ_diag_r n) => Hn.
+  destruct e;
+    repeat light || invert_constructor_equalities || destruct_match || eauto 3;
+    try solve [eapply_anywhere EvalListMaintained; eauto].
+  (** Only one case remaining *)
+  eapply H_trans with s; eauto.
+  eapply H_trans with s0; eauto.
+  eapply H_trans with (assign v1 v v2 s0); eauto.
+  unfold assign; repeat destruct_match; eauto using PeanoNat.Nat.eq_le_incl, update_one3.
+Qed.
