Compatibility.v
@@ -1,76 +1,70 @@
 From Celsius Require Export Trees Eval Reachability Tactics.
-Require Import ssreflect ssrbool.
-
-Require Import List.
+Require Import ssreflect ssrbool List.
 Import ListNotations.
 Open Scope nat_scope.
 
-Module Compatibility.
-  Import Eval.Evaluator.
-  Create HintDb cmpt.
+Create HintDb cmpt.
 
-  (* Definitions and notations : *)
-  Definition compatible (σ σ': Store) : Prop := forall l C ω,
-      getObj σ l  = Some (C, ω) ->
-      (exists ω', getObj σ' l = Some (C, ω')).
-  Notation "σ ⊆ σ'" := (compatible σ σ') (at level 80).
+(* Definitions and notations : *)
+Definition compatible (σ σ': Store) : Prop := forall l C ω,
+    getObj σ l  = Some (C, ω) ->
+    (exists ω', getObj σ' l = Some (C, ω')).
+Notation "σ ⊆ σ'" := (compatible σ σ') (at level 80).
 
-  Lemma compatibility_reflexivity : forall σ, σ ⊆ σ.
-  Proof.
-    unfold compatible. eauto. Qed.
-  Hint Resolve compatibility_reflexivity : cmpt.
+Lemma compatibility_reflexivity : forall σ, σ ⊆ σ.
+Proof.
+  unfold compatible. eauto. Qed.
+Hint Resolve compatibility_reflexivity : cmpt.
 
-  Lemma compatibility_transitivity : forall s1 s2 s3, s1 ⊆ s2 -> s2 ⊆ s3 -> s1 ⊆ s3.
-  Proof.
-    unfold compatible. intros.
-    move /(_ l C ω H1):H => [ω' H].
-    move /(_ l C ω' H):H0 => [ω'' H0].
+Lemma compatibility_transitivity : forall s1 s2 s3, s1 ⊆ s2 -> s2 ⊆ s3 -> s1 ⊆ s3.
+Proof.
+  unfold compatible. intros.
+  move /(_ l C ω H1):H => [ω' H].
+  move /(_ l C ω' H):H0 => [ω'' H0].
+  eauto.
+Qed.
+Hint Resolve compatibility_transitivity : cmpt.
+
+Lemma compatibility_assignment : forall (σ σ': Store) (l: Loc) (C: ClN) (ω ω': Env),
+    getObj σ l = Some (C, ω) ->
+    σ' = [l ↦ (C, ω')]σ ->
+    σ ⊆ σ'.
+Proof.
+  intros.
+  unfold compatible. intros.
+  move: (PeanoNat.Nat.eq_dec l l0) => [H4 | H4].
+  + rewrite H4 H1 in H.
+    invert_constructor_equalities.
+    rewrite H0 H4.
+    rewrite getObj_update1.
+    apply (getObj_dom _ _ _ H1).
+    exists ω' => //.
+  + rewrite H0.
+    rewrite getObj_update2.
+    apply (getObj_dom _ _ _ H).
     eauto.
-  Qed.
-  Hint Resolve compatibility_transitivity : cmpt.
+    exists ω0 => //.
+Qed.
+Hint Resolve compatibility_assignment: cmpt.
 
-  Lemma compatibility_assignment : forall (σ σ': Store) (l: Loc) (C: ClN) (ω ω': Env),
-      getObj σ l = Some (C, ω) ->
-      σ' = [l ↦ (C, ω')]σ ->
-      σ ⊆ σ'.
-  Proof.
-    intros.
-    unfold compatible. intros.
-    move: (PeanoNat.Nat.eq_dec l l0) => [H4 | H4].
-    + rewrite H4 H1 in H.
-      invert_constructor_equalities.
-      rewrite H0 H4.
-      rewrite getObj_update1.
-      apply (getObj_dom _ _ _ H1).
-      exists ω' => //.
-    + rewrite H0.
-      rewrite getObj_update2.
-      apply (getObj_dom _ _ _ H).
-      eauto.
-      exists ω0 => //.
-  Qed.
-  Hint Resolve compatibility_assignment: cmpt.
-
-  Lemma compatibility_freshness : forall (σ: Store) (c: ClN) (ρ: Env),
-      σ ⊆ σ ++ [(c, ρ)].
-  Proof.
-    unfold compatible.
-    induction σ; destruct l; simpl ; eauto => //.
-  Qed.
-  Hint Resolve compatibility_freshness: cmpt.
+Lemma compatibility_freshness : forall (σ: Store) (c: ClN) (ρ: Env),
+    σ ⊆ σ ++ [(c, ρ)].
+Proof.
+  unfold compatible.
+  induction σ; destruct l; simpl ; eauto => //.
+Qed.
+Hint Resolve compatibility_freshness: cmpt.
 
 
-  Lemma compatibility_InitMaintained: forall n,  InitMaintained compatible n.
-  Proof.
-    intros. apply freshnessInitMaintained; unfold Reflexive, Transitive, Assignment, Freshness; eauto with cmpt.
-  Qed.
-  Hint Resolve compatibility_InitMaintained: cmpt.
+Lemma compatibility_InitMaintained: forall n,  InitMaintained compatible n.
+Proof.
+  intros. apply FreshnessInitMaintained; unfold Reflexive, Transitive, Assignment, Freshness; eauto with cmpt.
+Qed.
+Hint Resolve compatibility_InitMaintained: cmpt.
 
 
-  Theorem compatibility_theorem: forall (n : nat), forall (e: Expr) (σ σ': Store) (ρ: Env) (v v': Value),
+Theorem compatibility_theorem: forall (n : nat), forall (e: Expr) (σ σ': Store) (ρ: Env) (v v': Value),
       ⟦e⟧(σ, ρ, v)(n) = (Success v' σ') -> σ ⊆ σ'.
-  Proof.
-    apply (eval_prop compatible); unfold Reflexive, Transitive, Assignment, Freshness; eauto with cmpt.
-  Qed.
-
-  End Compatibility.
+Proof.
+  apply (EvalMaintainedProp compatible); unfold Reflexive, Transitive, Assignment, Freshness; eauto with cmpt.
+Qed.
