PartialMonotonicity.v
@@ -1,154 +1,143 @@
 From Celsius Require Export Trees Eval Reachability Tactics Compatibility strongInduction.
-Require Import ssreflect ssrbool.
+Require Import ssreflect ssrbool List.
 
-
-Require Import List.
 Import ListNotations.
 Open Scope nat_scope.
 
-Module PartialMonotonicity.
-  Import Reachability.Reachability.
-  Import Eval.Evaluator.
-  Import Compatibility.Compatibility.
-  Create HintDb pM.
-  Hint Extern 1 => unfold dom in *: dm.
+Create HintDb pM.
+Hint Extern 1 => unfold dom in *: dm.
 
-  (* Definitions and notations : *)
-  Definition initializedFields (σ: Store) (l: Loc) (f: list Field) : Prop :=
-    match (getObj σ l) with
-    | Some (C, ω) => ((length f) <= (length ω))
-    | _ => False
-    end.
-  Notation "σ ⊨ l : f" := (initializedFields σ l f) (at level 80, l at level 80, f at level 80).
+(* Definitions and notations : *)
+Definition initializedFields (σ: Store) (l: Loc) (f: list Field) : Prop :=
+  match (getObj σ l) with
+  | Some (C, ω) => ((length f) <= (length ω))
+  | _ => False
+  end.
+Notation "σ ⊨ l : f" := (initializedFields σ l f) (at level 80, l at level 80, f at level 80).
 
-  Definition partialMonotonicity (σ σ': Store) :=
-    forall l f, (σ ⊨ l : f) -> (σ' ⊨ l : f).
-  Notation "σ ⪯ σ'" := (partialMonotonicity σ σ') (at level 80).
+Definition partialMonotonicity (σ σ': Store) :=
+  forall l f, (σ ⊨ l : f) -> (σ' ⊨ l : f).
+Notation "σ ⪯ σ'" := (partialMonotonicity σ σ') (at level 80).
 
 
-  (* Results : *)
+(* Results : *)
 
-  Lemma partialMonotonicity_reflexivity : forall (σ : Store), σ ⪯ σ.
-  Proof. unfold partialMonotonicity => //. Qed.
-  Hint Resolve partialMonotonicity_reflexivity: pM.
+Lemma partialMonotonicity_reflexivity : forall (σ : Store), σ ⪯ σ.
+Proof. unfold partialMonotonicity => //. Qed.
+Hint Resolve partialMonotonicity_reflexivity: pM.
 
-  Lemma initializedFields_dom : forall (σ: Store) (l: nat) (f: list Field), (σ ⊨ l : f) -> (l < (dom σ)).
-  Proof.
-    unfold initializedFields, getObj.
-    induction σ; repeat light || destruct l as [|l'] || eauto.
-      apply (PeanoNat.Nat.lt_0_succ).
-      apply (Lt.lt_n_S).
-      apply IHσ in H => //.
-  Qed.
-  Hint Resolve initializedFields_dom: pM.
+Lemma initializedFields_dom : forall (σ: Store) (l: nat) (f: list Field), (σ ⊨ l : f) -> (l < (dom σ)).
+Proof.
+  unfold initializedFields, getObj.
+  induction σ; repeat light || destruct l as [|l'] || eauto.
+  apply (PeanoNat.Nat.lt_0_succ).
+  apply (Lt.lt_n_S).
+  apply IHσ in H => //.
+Qed.
+Hint Resolve initializedFields_dom: pM.
 
-  Lemma initializedFields_exists : forall (σ: Store) (c: ClN) (e: Env), exists (f: list Field), ((c,e)::σ) ⊨ (dom σ) : f.
-  Proof.
-    unfold initializedFields.
-    intros. exists [].
-    induction σ; intros ; simpl ; eauto using le_0_n.
-    - destruct σ, a => //. apply le_0_n.
-  Qed.
+Lemma initializedFields_exists : forall (σ: Store) (c: ClN) (e: Env), exists (f: list Field), ((c,e)::σ) ⊨ (dom σ) : f.
+Proof.
+  unfold initializedFields.
+  intros. exists [].
+  induction σ; intros ; simpl ; eauto using le_0_n.
+  - destruct σ, a => //. apply le_0_n.
+Qed.
 
-  Lemma partialMonotonicity_domains : forall (σ σ': Store), σ ⪯ σ' -> (dom σ) <= (dom σ').
-  Proof.
-    intros.
-    unfold partialMonotonicity in H.
-    move : (initializedFields_dom σ') => Hσ'.
-    destruct (σ) eqn:Σ; eauto using le_0_n.
-    - destruct o.
-      case : (initializedFields_exists s c e) => f Hf.
-      eauto using Lt.lt_le_S.
-  Qed.
-  Hint Resolve partialMonotonicity_domains: pM.
-
-
-  Lemma partialMonotonicity_transitivity : forall (σ1 σ2 σ3 : Store), (σ1 ⪯ σ2) -> (σ2 ⪯ σ3) -> (σ1 ⪯ σ3).
-  Proof.
-    unfold partialMonotonicity; auto.
-  Qed.
-  Hint Resolve partialMonotonicity_transitivity: pM.
+Lemma partialMonotonicity_domains : forall (σ σ': Store), σ ⪯ σ' -> (dom σ) <= (dom σ').
+Proof.
+  intros.
+  unfold partialMonotonicity in H.
+  move : (initializedFields_dom σ') => Hσ'.
+  destruct (σ) eqn:Σ; eauto using le_0_n.
+  - destruct o.
+    case : (initializedFields_exists s c e) => f Hf.
+    eauto using Lt.lt_le_S.
+Qed.
+Hint Resolve partialMonotonicity_domains: pM.
 
 
-  Lemma partialMonotonicity_assignment : forall (σ σ': Store) (l: Loc) (C: ClN) (ω ω': Env),
-      getObj σ l = Some (C, ω) ->
-      length ω <= length ω' ->
-      σ' = [l ↦ (C, ω')]σ ->
-      σ ⪯ σ'.
-  Proof.
-    unfold partialMonotonicity, initializedFields.
-    intros.
-    move: (PeanoNat.Nat.eq_dec l l0) => [H4 | H4].
-    - rewrite H1 H4 getObj_update1 => //.
-      apply (initializedFields_dom _ _ f H2).
-      unfold initializedFields in H2.
-      rewrite -H4 H in H2 => //.
-      apply: (PeanoNat.Nat.le_trans _ _ _ H2 H0).
-    - move: (getObj_update2 σ (C, ω') l l0 ((getObj_dom σ (C,ω) l) H) H4)=>H5.
-      rewrite H1 H5 => //.
-  Qed.
-  Hint Resolve partialMonotonicity_assignment: pM.
+Lemma partialMonotonicity_transitivity : forall (σ1 σ2 σ3 : Store), (σ1 ⪯ σ2) -> (σ2 ⪯ σ3) -> (σ1 ⪯ σ3).
+Proof.
+  unfold partialMonotonicity; auto.
+Qed.
+Hint Resolve partialMonotonicity_transitivity: pM.
 
 
-  Lemma partialMonotonicity_freshness : forall (σ: Store) (c: ClN) (ρ: Env),
-      σ ⪯ σ ++ [(c, ρ)].
-  Proof.
-    unfold partialMonotonicity.
-    unfold initializedFields.
-    induction σ ; destruct l => //.
-    apply IHσ => //.
-  Qed.
-  Hint Resolve partialMonotonicity_freshness: pM.
+Lemma partialMonotonicity_assignment : forall (σ σ': Store) (l: Loc) (C: ClN) (ω ω': Env),
+    getObj σ l = Some (C, ω) ->
+    length ω <= length ω' ->
+    σ' = [l ↦ (C, ω')]σ ->
+    σ ⪯ σ'.
+Proof.
+  unfold partialMonotonicity, initializedFields.
+  intros.
+  move: (PeanoNat.Nat.eq_dec l l0) => [H4 | H4].
+  - rewrite H1 H4 getObj_update1 => //.
+    apply (initializedFields_dom _ _ f H2).
+    unfold initializedFields in H2.
+    rewrite -H4 H in H2 => //.
+    apply: (PeanoNat.Nat.le_trans _ _ _ H2 H0).
+  - move: (getObj_update2 σ (C, ω') l l0 ((getObj_dom σ (C,ω) l) H) H4)=>H5.
+    rewrite H1 H5 => //.
+Qed.
+Hint Resolve partialMonotonicity_assignment: pM.
 
-  Lemma partialMonotonicity_InitMaintained: forall n,  InitMaintained partialMonotonicity n.
-  Proof.
-    intros. apply freshnessInitMaintained; unfold Reflexive, Transitive, Assignment, Freshness; eauto with pM.
-  Qed.
-  Hint Resolve partialMonotonicity_InitMaintained: pM.
 
-  Theorem partialMonotonicity_theorem: forall (n : nat), forall (e: Expr) (σ σ': Store) (ρ: Env) (v v': Value),
+Lemma partialMonotonicity_freshness : forall (σ: Store) (c: ClN) (ρ: Env),
+    σ ⪯ σ ++ [(c, ρ)].
+Proof.
+  unfold partialMonotonicity.
+  unfold initializedFields.
+  induction σ ; destruct l => //.
+  apply IHσ => //.
+Qed.
+Hint Resolve partialMonotonicity_freshness: pM.
+
+Lemma partialMonotonicity_InitMaintained: forall n,  InitMaintained partialMonotonicity n.
+Proof.
+  intros. apply FreshnessInitMaintained; unfold Reflexive, Transitive, Assignment, Freshness; eauto with pM.
+Qed.
+Hint Resolve partialMonotonicity_InitMaintained: pM.
+
+Theorem partialMonotonicity_theorem: forall (n : nat), forall (e: Expr) (σ σ': Store) (ρ: Env) (v v': Value),
       ⟦e⟧(σ, ρ, v)(n) = (Success v' σ') -> σ ⪯ σ'.
-  Proof.
-    apply (eval_prop partialMonotonicity); unfold Reflexive, Transitive, Assignment, Freshness; eauto with pM.
+Proof.
+  apply (EvalMaintainedProp partialMonotonicity); unfold Reflexive, Transitive, Assignment, Freshness; eauto with pM.
 
-  Qed.
+Qed.
 
 
-  Theorem partialMonotonicity_theorem_dom: forall (n : nat), forall (e: Expr) (σ σ': Store) (ρ: Env) (v v': Value),
+Theorem partialMonotonicity_theorem_dom: forall (n : nat), forall (e: Expr) (σ σ': Store) (ρ: Env) (v v': Value),
       ⟦e⟧(σ, ρ, v)(n) = (Success v' σ') -> (dom σ) <= (dom σ').
-  Proof.
-    intros. apply partialMonotonicity_theorem in H.
-      by apply partialMonotonicity_domains.
-  Qed.
+Proof.
+  intros. apply partialMonotonicity_theorem in H.
+    by apply partialMonotonicity_domains.
+Qed.
 
-  Hint Resolve partialMonotonicity_theorem_dom: pM.
+Hint Resolve partialMonotonicity_theorem_dom: pM.
 
-  Theorem partialMonotonicity_theorem_list_dom: forall n el σ σ' ρ ψ ρ',
-      ⟦_ el _⟧(σ, ρ, ψ)(n) = (Success_l ρ' σ') -> (dom σ) <= (dom σ').
-  Proof.
-    intros.
-    eapply (eval_list_prop (fun σ σ' => dom σ <= dom σ') (S n)); intros;
-      unfold Reflexive, Transitive, Assignment, Freshness, EvalMaintained; eauto with pM lia.
-  Qed.
-  Hint Resolve partialMonotonicity_theorem_list_dom: pM.
-
-
-
-  Lemma partialMonotonicity_warm_monotone: forall σ σ' l, σ ⪯ σ' -> σ ⊆ σ' -> (σ ⊨ l : warm) -> (σ' ⊨ l : warm).
-  Proof.
-    unfold reachable_warm.
-    intros σ σ' l H_pm H_c [C [ω [args [fields[ methods [H2 [H3 H4]] ]]]]].
-    unfold partialMonotonicity, initializedFields in H_pm.
-    move /(_ l fields):H_pm => H_pm.
-    rewrite H2 in H_pm.
-    move /(_ H4):H_pm => H_pm.
-    unfold compatible in H_c.
-    move /(_ l C ω H2):H_c => [ω' H_c].
-    rewrite H_c in H_pm.
-    exists C, ω', args, fields, methods => //.
-  Qed.
+Theorem partialMonotonicity_theorem_list_dom: forall n el σ σ' ρ ψ ρ',
+    ⟦_ el _⟧(σ, ρ, ψ)(n) = (Success_l ρ' σ') -> (dom σ) <= (dom σ').
+Proof.
+  intros.
+  eapply (EvalListMaintained (fun σ σ' => dom σ <= dom σ') (S n)); intros;
+    unfold Reflexive, Transitive, Assignment, Freshness, EvalMaintained; eauto with pM lia.
+Qed.
+Hint Resolve partialMonotonicity_theorem_list_dom: pM.
 
 
 
-
-End PartialMonotonicity.
+Lemma partialMonotonicity_warm_monotone: forall σ σ' l, σ ⪯ σ' -> σ ⊆ σ' -> (σ ⊨ l : warm) -> (σ' ⊨ l : warm).
+Proof.
+  unfold reachable_warm.
+  intros σ σ' l H_pm H_c [C [ω [args [fields[ methods [H2 [H3 H4]] ]]]]].
+  unfold partialMonotonicity, initializedFields in H_pm.
+  move /(_ l fields):H_pm => H_pm.
+  rewrite H2 in H_pm.
+  move /(_ H4):H_pm => H_pm.
+  unfold compatible in H_c.
+  move /(_ l C ω H2):H_c => [ω' H_c].
+  rewrite H_c in H_pm.
+  exists C, ω', args, fields, methods => //.
+Qed.
