Reachability.v
@@ -1,80 +1,78 @@
-From Celsius Require Export Trees.
-From Celsius Require Export Eval.
+From Celsius Require Export Trees Eval.
 
 Require Import ssreflect ssrbool.
-
 Require Import Coq.Arith.Wf_nat.
 Require Import Coq.Wellfounded.Wellfounded.
 Require Import List.
-Import ListNotations.
-Open Scope nat_scope.
-Open Scope list_scope.
 Require Import Sets.Ensembles.
 Require Import Psatz.
 
-Module Reachability.
-  Import Eval.Evaluator.
+Import ListNotations.
+Open Scope nat_scope.
+Open Scope list_scope.
 
-  Reserved Notation "σ ⊨ l1 ⇝ l2" (at level 80, l1 at level 80, l2 at level 80).
-  Inductive reachability : Store -> Loc -> Loc ->Prop :=
-  | rch_heap:
-      forall l σ,
-        l < (dom σ) ->
-        σ ⊨ l ⇝ l
-  | rch_step:
-      forall l0 l1 C f ω σ,
-        l1 < (dom σ) ->
-        getObj σ l0 = Some (C, ω) ->
-        getVal ω f = Some l1 ->
-        σ ⊨ l0 ⇝ l1
-  | rch_trans:
-      forall l0 l1 l2 σ,
-        σ ⊨ l0 ⇝ l1 ->
-        σ ⊨ l1 ⇝ l2 ->
-        σ ⊨ l0 ⇝ l2
-  where "σ ⊨ l1 ⇝ l2" := (reachability σ l1 l2).
-  Hint Resolve rch_heap rch_step rch_trans: rch.
-  Hint Rewrite update_dom: rch.
 
-  Definition reachability_set σ (L: LocSet) l := exists l', (l' ∈ L) /\ (σ ⊨ l' ⇝ l).
-  Notation "σ ⊫ L ⇝ l" := (reachability_set σ L l) (at level 80, l at level 99, L at level 99).
+Reserved Notation "σ ⊨ l1 ⇝ l2" (at level 80, l1 at level 80, l2 at level 80).
+Inductive reachability : Store -> Loc -> Loc ->Prop :=
+| rch_heap:
+    forall l σ,
+      l < (dom σ) ->
+      σ ⊨ l ⇝ l
+| rch_step:
+    forall l0 l1 C f ω σ,
+      l1 < (dom σ) ->
+      getObj σ l0 = Some (C, ω) ->
+      getVal ω f = Some l1 ->
+      σ ⊨ l0 ⇝ l1
+| rch_trans:
+    forall l0 l1 l2 σ,
+      σ ⊨ l0 ⇝ l1 ->
+      σ ⊨ l1 ⇝ l2 ->
+      σ ⊨ l0 ⇝ l2
+where "σ ⊨ l1 ⇝ l2" := (reachability σ l1 l2).
 
-  Definition reachable_cold (σ: Store) (l: Loc) := (l < dom σ).
-  Notation "σ ⊨ l : 'cold'" := (reachable_cold σ l) (at level 80, l at level 80).
-  Notation "σ ⊫ L : 'cold'" := (forall l, (l ∈ L) -> reachable_cold σ l) (at level 80, L at level 99).
+Hint Resolve rch_heap rch_step rch_trans: rch.
+Hint Rewrite update_dom: rch.
 
-  Definition reachable_warm (σ: Store) (l: Loc) := (exists C ω args fields methods , (getObj σ l) = Some (C, ω) /\ ((ct C) = Some (class args fields methods)) /\ (length fields <= length ω)).
-  Notation "σ ⊨ l : 'warm'" := (reachable_warm σ l) (at level 80, l at level 80).
-  Notation "σ ⊫ L : 'warm'" := (forall l, (l ∈ L) -> reachable_warm σ l) (at level 80, L at level 99).
+Definition reachability_set σ (L: LocSet) l := exists l', (l' ∈ L) /\ (σ ⊨ l' ⇝ l).
+Notation "σ ⊫ L ⇝ l" := (reachability_set σ L l) (at level 80, l at level 99, L at level 99).
 
-  Definition reachable_hot  (σ: Store) (l: Loc) :=(forall (l': Loc), (σ ⊨ l ⇝ l') -> (σ ⊨ l' : warm)).
-  Notation "σ ⊨ l : 'hot'"  := (reachable_hot σ l) (at level 80, l at level 80).
-  Notation "σ ⊫ L : 'hot'" := (forall l, (l ∈ L) -> reachable_hot σ l) (at level 80, L at level 99).
+Definition reachable_cold (σ: Store) (l: Loc) := (l < dom σ).
+Notation "σ ⊨ l : 'cold'" := (reachable_cold σ l) (at level 80, l at level 80).
+Notation "σ ⊫ L : 'cold'" := (forall l, (l ∈ L) -> reachable_cold σ l) (at level 80, L at level 99).
 
-  Lemma reachability_trans: (forall σ l1 l2 l3, (σ ⊨ l1 ⇝ l2) -> (σ ⊨ l2 ⇝ l3) -> (σ ⊨ l1 ⇝ l3)).
-  Proof.
-    eauto using rch_trans.
-  Qed.
+Definition reachable_warm (σ: Store) (l: Loc) := (exists C ω args fields methods , (getObj σ l) = Some (C, ω) /\ ((ct C) = Some (class args fields methods)) /\ (length fields <= length ω)).
+Notation "σ ⊨ l : 'warm'" := (reachable_warm σ l) (at level 80, l at level 80).
+Notation "σ ⊫ L : 'warm'" := (forall l, (l ∈ L) -> reachable_warm σ l) (at level 80, L at level 99).
 
-  Lemma reachability_hot: forall (σ: Store) (l l': Loc), σ ⊨ l: hot -> σ ⊨ l ⇝ l' -> σ ⊨ l': hot.
-  Proof.
-    intros σ l l' H1 H2 l'' H3.
-    apply (H1 l'' ((reachability_trans _ _ _ _) H2 H3)).
-  Qed.
+Definition reachable_hot  (σ: Store) (l: Loc) :=(forall (l': Loc), (σ ⊨ l ⇝ l') -> (σ ⊨ l' : warm)).
+Notation "σ ⊨ l : 'hot'"  := (reachable_hot σ l) (at level 80, l at level 80).
+Notation "σ ⊫ L : 'hot'" := (forall l, (l ∈ L) -> reachable_hot σ l) (at level 80, L at level 99).
 
-  Lemma reachability_singleton : forall σ l1 l2, (σ ⊫ (Singleton Loc l1) ⇝ l2) <-> σ ⊨ l1 ⇝ l2.
-  Proof.
-    split; intros.
-    unfold reachability_set in H. repeat destruct H => //.
-    exists l1 => //.
-  Qed.
+Lemma reachability_trans: (forall σ l1 l2 l3, (σ ⊨ l1 ⇝ l2) -> (σ ⊨ l2 ⇝ l3) -> (σ ⊨ l1 ⇝ l3)).
+Proof.
+  eauto using rch_trans.
+Qed.
 
-  Lemma reachability_dom : forall σ l1 l2, (σ ⊨ l1 ⇝ l2) -> (l1 < (dom σ)) /\ (l2 < (dom σ)).
-    intros.
-    induction H; repeat steps || eapply_anywhere getObj_dom.
-  Qed.
+Lemma reachability_hot: forall (σ: Store) (l l': Loc), σ ⊨ l: hot -> σ ⊨ l ⇝ l' -> σ ⊨ l': hot.
+Proof.
+  intros σ l l' H1 H2 l'' H3.
+  apply (H1 l'' ((reachability_trans _ _ _ _) H2 H3)).
+Qed.
 
-  (*
+Lemma reachability_singleton : forall σ l1 l2, (σ ⊫ (Singleton Loc l1) ⇝ l2) <-> σ ⊨ l1 ⇝ l2.
+Proof.
+  split; intros.
+  unfold reachability_set in H. repeat destruct H => //.
+  exists l1 => //.
+Qed.
+
+Lemma reachability_dom : forall σ l1 l2, (σ ⊨ l1 ⇝ l2) -> (l1 < (dom σ)) /\ (l2 < (dom σ)).
+  intros.
+  induction H; repeat steps || eapply_anywhere getObj_dom.
+Qed.
+
+(*
   Lemma reachability_rev:
     forall σ l l',
       σ ⊨ l ⇝ l' ->
@@ -87,399 +85,396 @@ Module Reachability.
     + right. repeat eexists; eauto using rch_heap, rch_trans.
   Qed. *)
 
-  Lemma reachability_rev_ind:
-    forall (P: Loc -> Loc -> Prop) σ,
-      (forall l, l < dom σ -> P l l) ->
-      (forall l1 l2 l3, P l1 l2 -> P l2 l3 -> P l1 l3) ->
-      (forall l l' C ω f , l' < dom σ -> getObj σ l = Some(C, ω) /\ getVal ω f = Some l' -> P l l') ->
-      (forall l l', σ ⊨ l ⇝ l' -> P l l').
-  Proof.
-    intros.
-    induction H2; eauto.
-  Qed.
+Lemma reachability_rev_ind:
+  forall (P: Loc -> Loc -> Prop) σ,
+    (forall l, l < dom σ -> P l l) ->
+    (forall l1 l2 l3, P l1 l2 -> P l2 l3 -> P l1 l3) ->
+    (forall l l' C ω f , l' < dom σ -> getObj σ l = Some(C, ω) /\ getVal ω f = Some l' -> P l l') ->
+    (forall l l', σ ⊨ l ⇝ l' -> P l l').
+Proof.
+  intros.
+  induction H2; eauto.
+Qed.
 
-  Lemma reachability_add_env:
-    forall σ x C ω l,
-      x < dom σ ->
-      getObj σ x = Some(C, ω) ->
-      forall l1 l2,
-        ([x ↦ (C, ω ++ [l])]σ) ⊨ l1 ⇝ l2 ->
-        σ ⊨ l1 ⇝ l2 \/ ((σ ⊨ l1 ⇝ x) /\ σ ⊨ l ⇝ l2).
-  Proof.
-    intros σ x C ω l Hx Hobj.
-    apply reachability_rev_ind; steps; eauto with rch;
-      rewrite_anywhere update_dom; eauto with rch.
-    eapply_anywhere getObj_update3; steps; eauto with rch.
-    eapply_anywhere getVal_add; steps; eauto with rch.
-  Qed.
-
-
-  Lemma reachability_weaken_assignment :
-    forall σ σ' C ω ω' s e f l l',
-      (getObj σ l) = Some (C, ω) ->
-      ω' = [f ↦ l']ω ->
-      σ' = [l ↦ (C, ω')]σ ->
-      (l = l') ->
-      σ' ⊨ s ⇝ e ->
-      σ ⊨ s ⇝ e.
-  Proof.
-    intros. move: H3. move: s e. induction 1; repeat steps || rewrite_anywhere update_dom; eauto with rch.
-    eapply_anywhere getObj_update3; eauto using getObj_dom; steps; eauto with rch.
-    eapply_anywhere getVal_update; steps;  eauto with rch.
-  Qed.
-
-  (* Notions of path into the heap *)
-
-  Definition reachable_one_step σ l0 l1 :=
-    exists C ω, (getObj σ l0 = Some (C, ω)) /\ (exists f, (getVal ω f = Some l1)) /\ (l1 < dom σ).
+Lemma reachability_add_env:
+  forall σ x C ω l,
+    x < dom σ ->
+    getObj σ x = Some(C, ω) ->
+    forall l1 l2,
+      ([x ↦ (C, ω ++ [l])]σ) ⊨ l1 ⇝ l2 ->
+      σ ⊨ l1 ⇝ l2 \/ ((σ ⊨ l1 ⇝ x) /\ σ ⊨ l ⇝ l2).
+Proof.
+  intros σ x C ω l Hx Hobj.
+  apply reachability_rev_ind; steps; eauto with rch;
+    rewrite_anywhere update_dom; eauto with rch.
+  eapply_anywhere getObj_update3; steps; eauto with rch.
+  eapply_anywhere getVal_add; steps; eauto with rch.
+Qed.
 
 
-  Lemma reachable_one_step_reachability :
-    forall σ l0 l1, reachable_one_step σ l0 l1 -> σ ⊨ l0 ⇝ l1.
-  Proof.
-    unfold reachable_one_step; steps.
+Lemma reachability_weaken_assignment :
+  forall σ σ' C ω ω' s e f l l',
+    (getObj σ l) = Some (C, ω) ->
+    ω' = [f ↦ l']ω ->
+    σ' = [l ↦ (C, ω')]σ ->
+    (l = l') ->
+    σ' ⊨ s ⇝ e ->
+    σ ⊨ s ⇝ e.
+Proof.
+  intros. move: H3. move: s e. induction 1; repeat steps || rewrite_anywhere update_dom; eauto with rch.
+  eapply_anywhere getObj_update3; eauto using getObj_dom; steps; eauto with rch.
+  eapply_anywhere getVal_update; steps;  eauto with rch.
+Qed.
+
+(* Notions of path into the heap *)
+
+Definition reachable_one_step σ l0 l1 :=
+  exists C ω, (getObj σ l0 = Some (C, ω)) /\ (exists f, (getVal ω f = Some l1)) /\ (l1 < dom σ).
+
+
+Lemma reachable_one_step_reachability :
+  forall σ l0 l1, reachable_one_step σ l0 l1 -> σ ⊨ l0 ⇝ l1.
+Proof.
+  unfold reachable_one_step; steps.
+  eauto with rch.
+Qed.
+Hint Resolve reachable_one_step_reachability : rch.
+
+(* Path in σ (p is in reverse order) *)
+Fixpoint reachable_path σ p {struct p}:=
+  match p with
+  | [] => True
+  | l1::nil => l1 < dom σ
+  | l2::((l1::_) as p') => reachable_one_step σ l1 l2 /\ reachable_path σ p'
+  end.
+
+Definition contains_edge p (l1 l2 :Loc) :=
+  exists p1 p2, p = p2 ++ l2::l1::p1.
+
+
+Lemma reachable_path_trans:
+  forall σ p1 p2 l,
+    reachable_path σ (p1++[l]) ->
+    reachable_path σ (l::p2) ->
+    reachable_path σ (p1++(l::p2)).
+Proof.
+  induction p1; [steps | intros].
+  simpl. simpl in H.
+  repeat (destruct_match; [destruct p1; steps |]).
+  assert (n0 = n) by (destruct p1; steps); subst.
+  destruct_and.
+  split; eauto.
+  rewrite_back_any.
+  eapply IHp1; eauto. rewrite_any => //.
+Qed.
+
+
+Lemma reachable_path_reachability:
+  forall σ s e,
+    ((s = e /\ s < dom σ) \/ exists p, reachable_path σ (e :: (p++[s]))) <-> σ ⊨ s ⇝ e.
+Proof.
+  split.
+  + intros [[H1 H2] | [p Hp]]; subst; eauto with rch.
+    generalize dependent e.
+    induction p; repeat light; eauto using reachable_one_step_reachability.
+    specialize (IHp a).
+    unfold reachable_one_step in H. destructs.
     eauto with rch.
-  Qed.
-  Hint Resolve reachable_one_step_reachability : rch.
-
-  (* Path in σ (p is in reverse order) *)
-  Fixpoint reachable_path σ p {struct p}:=
-    match p with
-    | [] => True
-    | l1::nil => l1 < dom σ
-    | l2::((l1::_) as p') => reachable_one_step σ l1 l2 /\ reachable_path σ p'
-    end.
-
-  Definition contains_edge p (l1 l2 :Loc) :=
-    exists p1 p2, p = p2 ++ l2::l1::p1.
+  + induction 1; destructs; eauto; right.
+    ++ exists []; simpl; unfold reachable_one_step.
+       repeat eexists; eauto using getObj_dom.
+    ++ exists (p++(l1::p0)).
+       rewrite <- app_assoc, app_comm_cons.
+       eauto using reachable_path_trans, app_comm_cons.
+Qed.
 
 
-  Lemma reachable_path_trans:
-    forall σ p1 p2 l,
-      reachable_path σ (p1++[l]) ->
-      reachable_path σ (l::p2) ->
-      reachable_path σ (p1++(l::p2)).
-  Proof.
-    induction p1; [steps | intros].
-    simpl. simpl in H.
-    repeat (destruct_match; [destruct p1; steps |]).
-    assert (n0 = n) by (destruct p1; steps); subst.
+Lemma reachable_path_is_reachable:
+  forall σ p e l,
+    reachable_path σ (e::p) ->
+    List.In l (e::p) ->
+    σ ⊨ l ⇝ e.
+Proof.
+  induction p ; try solve [repeat light ; eauto using rch_heap].
+  intros. destruct H0 as [H0 | H0]; subst.
+  + destruct p eqn:P ; repeat light;
+      apply reachable_one_step_reachability, reachability_dom in H0;
+      apply rch_heap; steps.
+  + move /(_ a l):IHp => IHp.
+    destruct p eqn:P; [steps; eauto with rch|].
+    rewrite <- P in *. simpl in H.
     destruct_and.
-    split; eauto.
-    rewrite_back_any.
-    eapply IHp1; eauto. rewrite_any => //.
-  Qed.
+    unfold reachable_one_step in H.
+    destructs.
+    eapply rch_trans with a; eauto with rch.
+    eapply IHp => //.
+Qed.
 
 
-  Lemma reachable_path_reachability:
-    forall σ s e,
-      ((s = e /\ s < dom σ) \/ exists p, reachable_path σ (e :: (p++[s]))) <-> σ ⊨ s ⇝ e.
-  Proof.
-    split.
-    + intros [[H1 H2] | [p Hp]]; subst; eauto with rch.
-      generalize dependent e.
-      induction p; repeat light; eauto using reachable_one_step_reachability.
-      specialize (IHp a).
-      unfold reachable_one_step in H. destructs.
-      eauto with rch.
-    + induction 1; destructs; eauto; right.
-      ++ exists []; simpl; unfold reachable_one_step.
-         repeat eexists; eauto using getObj_dom.
-      ++ exists (p++(l1::p0)).
-         rewrite <- app_assoc, app_comm_cons.
-         eauto using reachable_path_trans, app_comm_cons.
-  Qed.
+Lemma reachable_path_last:
+  forall σ s1 s2 p,
+    reachable_path σ (p++[s2;s1]) ->
+    reachable_path σ (p++[s2]).
+Proof.
+  induction p; simpl in *.
+  + unfold reachable_one_step in * ; steps.
+  + repeat (destruct_match; [ apply_anywhere app_eq_nil; steps | ]).
+    assert ( n = n0) by (destruct p; steps); steps.
+Qed.
 
 
-  Lemma reachable_path_is_reachable:
-    forall σ p e l,
-      reachable_path σ (e::p) ->
-      List.In l (e::p) ->
-      σ ⊨ l ⇝ e.
-  Proof.
-    induction p ; try solve [repeat light ; eauto using rch_heap].
-    intros. destruct H0 as [H0 | H0]; subst.
-    + destruct p eqn:P ; repeat light;
-        apply reachable_one_step_reachability, reachability_dom in H0;
-        apply rch_heap; steps.
-    + move /(_ a l):IHp => IHp.
-      destruct p eqn:P; [steps; eauto with rch|].
-      rewrite <- P in *. simpl in H.
-      destruct_and.
-      unfold reachable_one_step in H.
-      destructs.
-        eapply rch_trans with a; eauto with rch.
-        eapply IHp => //.
-  Qed.
+Lemma reachable_path_app:
+  forall σ s1 s2 p1 p2,
+    reachable_path σ (p2++s2::p1++[s1]) ->
+    reachable_path σ (s2::p1++[s1]) /\ reachable_path σ (p2++[s2]).
+Proof.
+  split.
+  + move: H. move: s1 s2 p1.
+    induction p2; simpl.
+    ++ destruct p1; steps.
+    ++ intros. repeat ( destruct_match; [apply_anywhere app_eq_nil; steps |]).
+       repeat rewrite_back_any.
+       steps; eapply_anywhere IHp2; steps.
+  + assert (forall l p s, reachable_path σ (p++s::l) -> reachable_path σ (p++[s])); eauto.
+    induction l; steps.
+    specialize (IHl (p++[s]) a).
+    eapply reachable_path_last.
+    repeat rewrite <- app_assoc in *.
+    simpl in *; eauto.
+Qed.
+
+Lemma app_exists_last:
+  forall p (x:Loc),
+  exists y p', x::p = p'++[y].
+Proof.
+  induction p; steps.
+  + exists x, []; steps.
+  + move /(_ a):IHp => IHp. steps.
+    exists y, (x::p'); steps.
+Qed.
 
 
-  Lemma reachable_path_last:
-    forall σ s1 s2 p,
-      reachable_path σ (p++[s2;s1]) ->
-      reachable_path σ (p++[s2]).
-  Proof.
-    induction p; simpl in *.
-    + unfold reachable_one_step in * ; steps.
-    + repeat (destruct_match; [ apply_anywhere app_eq_nil; steps | ]).
-      assert ( n = n0) by (destruct p; steps); steps.
-  Qed.
-
-
-  Lemma reachable_path_app:
-    forall σ s1 s2 p1 p2,
-      reachable_path σ (p2++s2::p1++[s1]) ->
-      reachable_path σ (s2::p1++[s1]) /\ reachable_path σ (p2++[s2]).
-  Proof.
-    split.
-    + move: H. move: s1 s2 p1.
-      induction p2; simpl.
-      ++ destruct p1; steps.
-      ++ intros. repeat ( destruct_match; [apply_anywhere app_eq_nil; steps |]).
-         repeat rewrite_back_any.
-         steps; eapply_anywhere IHp2; steps.
-    + assert (forall l p s, reachable_path σ (p++s::l) -> reachable_path σ (p++[s])); eauto.
-      induction l; steps.
-      specialize (IHl (p++[s]) a).
-      eapply reachable_path_last.
-      repeat rewrite <- app_assoc in *.
-      simpl in *; eauto.
-  Qed.
-
-  Lemma app_exists_last:
-    forall p (x:Loc),
-    exists y p', x::p = p'++[y].
-  Proof.
-    induction p; steps.
-    + exists x, []; steps.
-    + move /(_ a):IHp => IHp. steps.
-      exists y, (x::p'); steps.
-  Qed.
-
-
-  Lemma reachable_path_app2:
-    forall σ s p1 p2,
-      reachable_path σ (p2++s::p1) ->
-      reachable_path σ (p2++[s]).
-  Proof.
-    assert (
-        forall (σ : list Obj) (s s': nat) (p1 p2 : list nat),
-          reachable_path σ (p2 ++ s :: p1++[s']) -> reachable_path σ (p2 ++ [s])) by
-        repeat steps || eapply_anywhere reachable_path_app.
-    intros.
-    destruct p1 => //.
-    pose proof (app_exists_last p1 n) ; steps.
-    rewrite H1 in H0; eauto.
-  Qed.
+Lemma reachable_path_app2:
+  forall σ s p1 p2,
+    reachable_path σ (p2++s::p1) ->
+    reachable_path σ (p2++[s]).
+Proof.
+  assert (
+      forall (σ : list Obj) (s s': nat) (p1 p2 : list nat),
+        reachable_path σ (p2 ++ s :: p1++[s']) -> reachable_path σ (p2 ++ [s])) by
+      repeat steps || eapply_anywhere reachable_path_app.
+  intros.
+  destruct p1 => //.
+  pose proof (app_exists_last p1 n) ; steps.
+  rewrite H1 in H0; eauto.
+Qed.
 
 
 
-  Lemma contains_edge_dec :
-    forall p l1 l2, contains_edge p l1 l2 \/ not (contains_edge p l1 l2).
-  Proof.
-    unfold contains_edge. intros.
-    induction p; steps.
-    + right. steps. symmetry in H. apply app_eq_nil in H. steps.
-    + left. exists p1, (a::p2); steps.
-    + destruct (PeanoNat.Nat.eq_dec a l2) as [Ha | Ha]; subst.
-      ++ (* a = l2 *)
-        destruct p; steps.
-        +++ right; steps. symmetry in H0. apply app_eq_unit in H0; steps.
-        +++ destruct (PeanoNat.Nat.eq_dec l l1) as [Hl | Hl];
-              [ left | right]; steps;
-                [ exists p, [] | destruct p2] ; steps; eauto.
-      ++ right; steps.
-         destruct p2; steps; eauto.
-  Qed.
+Lemma contains_edge_dec :
+  forall p l1 l2, contains_edge p l1 l2 \/ not (contains_edge p l1 l2).
+Proof.
+  unfold contains_edge. intros.
+  induction p; steps.
+  + right. steps. symmetry in H. apply app_eq_nil in H. steps.
+  + left. exists p1, (a::p2); steps.
+  + destruct (PeanoNat.Nat.eq_dec a l2) as [Ha | Ha]; subst.
+    ++ (* a = l2 *)
+      destruct p; steps.
+      +++ right; steps. symmetry in H0. apply app_eq_unit in H0; steps.
+      +++ destruct (PeanoNat.Nat.eq_dec l l1) as [Hl | Hl];
+            [ left | right]; steps;
+              [ exists p, [] | destruct p2] ; steps; eauto.
+    ++ right; steps.
+       destruct p2; steps; eauto.
+Qed.
 
 
-  Lemma contains_edge_cons :
-    forall p l l' l0,
-      contains_edge (l0::p) l l' ->
-      l' <> l0 ->
-      contains_edge p l l'.
-  Proof.
-    unfold contains_edge; steps.
-    destruct p2; steps; eauto.
-  Qed.
+Lemma contains_edge_cons :
+  forall p l l' l0,
+    contains_edge (l0::p) l l' ->
+    l' <> l0 ->
+    contains_edge p l l'.
+Proof.
+  unfold contains_edge; steps.
+  destruct p2; steps; eauto.
+Qed.
 
 
-  Lemma reachable_path_split_on_edge:
-    forall σ s p l1 l2,
-      reachable_path σ (p++[s]) ->
-      contains_edge p l1 l2 ->
-      σ ⊨ s ⇝ l1.
-  Proof.
-    unfold contains_edge; steps.
-    move: H. move: l1 l2 p1.
-    induction p2; intros; simpl in *.
-    + eapply reachable_path_is_reachable; destructs; eauto.
-      rewrite app_comm_cons. apply in_app_iff; steps.
-    + destruct_match; [apply_anywhere app_eq_nil; steps |].
-      rewrite <- matched in *. destructs; eauto.
-  Qed.
+Lemma reachable_path_split_on_edge:
+  forall σ s p l1 l2,
+    reachable_path σ (p++[s]) ->
+    contains_edge p l1 l2 ->
+    σ ⊨ s ⇝ l1.
+Proof.
+  unfold contains_edge; steps.
+  move: H. move: l1 l2 p1.
+  induction p2; intros; simpl in *.
+  + eapply reachable_path_is_reachable; destructs; eauto.
+    rewrite app_comm_cons. apply in_app_iff; steps.
+  + destruct_match; [apply_anywhere app_eq_nil; steps |].
+    rewrite <- matched in *. destructs; eauto.
+Qed.
 
 
-  Lemma contains_edge_assignment :
-    forall σ σ' C ω ω' p f l l',
-      (getObj σ l) = Some (C, ω) ->
-      ω' = [f ↦ l']ω ->
-      σ' = [l ↦ (C, ω')]σ ->
-      not (contains_edge p l l') ->
-      reachable_path σ' p ->
-      reachable_path σ p.
-  Proof.
-    intros.
-    generalize dependent p.
-    induction p as [| l2 p]; intros; simpl; eauto.
-    destruct p as [| l1 p]; [ simpl in *; subst; unfold dom in *; rewrite_anywhere update_one3; eauto |].
-    simpl in H3. destruct_and.
-    split.
-    + unfold reachable_one_step in *; destructs.
-      repeat rewrite_anywhere update_dom.
-      destruct (PeanoNat.Nat.eq_dec l1 l); subst.
-      ++ rewrite_anywhere getObj_update1; eauto using getObj_dom.
-         invert_constructor_equalities; subst.
-         destruct (PeanoNat.Nat.eq_dec l2 l'); subst ; [exfalso; apply H2; exists p, []  ; steps |].
-         unfold getVal in *. exists C0, ω; repeat split; eauto.
-         destruct (PeanoNat.Nat.eq_dec f f0); subst; rewrite_anywhere  update_one2; eauto.
-         apply_anywhere update_one4; subst. congruence.
-      ++ rewrite_anywhere getObj_update2; eauto using getObj_dom.
-         repeat eexists || split || eauto.
-    + apply IHp; eauto.
-      intros [p1 [p2 Hedge]].
-      apply H2. exists p1, (l2::p2).
-      rewrite Hedge; eauto.
-  Qed.
+Lemma contains_edge_assignment :
+  forall σ σ' C ω ω' p f l l',
+    (getObj σ l) = Some (C, ω) ->
+    ω' = [f ↦ l']ω ->
+    σ' = [l ↦ (C, ω')]σ ->
+    not (contains_edge p l l') ->
+    reachable_path σ' p ->
+    reachable_path σ p.
+Proof.
+  intros.
+  generalize dependent p.
+  induction p as [| l2 p]; intros; simpl; eauto.
+  destruct p as [| l1 p]; [ simpl in *; subst; unfold dom in *; rewrite_anywhere update_one3; eauto |].
+  simpl in H3. destruct_and.
+  split.
+  + unfold reachable_one_step in *; destructs.
+    repeat rewrite_anywhere update_dom.
+    destruct (PeanoNat.Nat.eq_dec l1 l); subst.
+    ++ rewrite_anywhere getObj_update1; eauto using getObj_dom.
+       invert_constructor_equalities; subst.
+       destruct (PeanoNat.Nat.eq_dec l2 l'); subst ; [exfalso; apply H2; exists p, []  ; steps |].
+       unfold getVal in *. exists C0, ω; repeat split; eauto.
+       destruct (PeanoNat.Nat.eq_dec f f0); subst; rewrite_anywhere  update_one2; eauto.
+       apply_anywhere update_one4; subst. congruence.
+    ++ rewrite_anywhere getObj_update2; eauto using getObj_dom.
+       repeat eexists || split || eauto.
+  + apply IHp; eauto.
+    intros [p1 [p2 Hedge]].
+    apply H2. exists p1, (l2::p2).
+    rewrite Hedge; eauto.
+Qed.
 
 
-  Lemma contains_edge_first_edge :
-    forall p l l',
-      contains_edge p l l' ->
-      exists p1 p2, p = p1++(l'::l::p2) /\ not (contains_edge p2 l l').
-  Proof.
-    induction p as [p IHp] using (induction_ltof1 _ (fun x => length x)); unfold ltof in IHp.
-    intros l l' [p1 [p2 H]].
-    destruct (contains_edge_dec p1 l l').
-    + apply IHp in H0.
-      destruct H0 as [p3 [p4 [H01 H02]]].
-      subst. exists (p2 ++ l' :: l :: p3), p4; split; eauto.
-      repeat rewrite app_comm_cons || rewrite app_assoc => //.
-      subst. rewrite app_length; simpl. Psatz.lia.
-    + exists p2, p1; split; eauto.
-  Qed.
+Lemma contains_edge_first_edge :
+  forall p l l',
+    contains_edge p l l' ->
+    exists p1 p2, p = p1++(l'::l::p2) /\ not (contains_edge p2 l l').
+Proof.
+  induction p as [p IHp] using (induction_ltof1 _ (fun x => length x)); unfold ltof in IHp.
+  intros l l' [p1 [p2 H]].
+  destruct (contains_edge_dec p1 l l').
+  + apply IHp in H0.
+    destruct H0 as [p3 [p4 [H01 H02]]].
+    subst. exists (p2 ++ l' :: l :: p3), p4; split; eauto.
+    repeat rewrite app_comm_cons || rewrite app_assoc => //.
+    subst. rewrite app_length; simpl. Psatz.lia.
+  + exists p2, p1; split; eauto.
+Qed.
 
-  Lemma contains_edge_last_edge :
-    forall p l l',
-      contains_edge p l l' ->
-      exists p1 p2, p = p1++(l'::l::p2) /\ not (contains_edge p1 l l').
-  Proof.
-    induction p as [p IHp] using (induction_ltof1 _ (fun x => length x)); unfold ltof in IHp.
-    intros l l' [p1 [p2 H]].
-    destruct (contains_edge_dec p2 l l').
-    + apply IHp in H0.
-      destruct H0 as [p3 [p4 [H01 H02]]].
-      subst. exists p3 , (p4 ++ l' :: l :: p1) ; split; eauto.
-      repeat rewrite app_comm_cons || rewrite app_assoc => //.
-      subst. rewrite app_length; simpl. Psatz.lia.
-    + exists p2, p1; split; eauto.
-  Qed.
+Lemma contains_edge_last_edge :
+  forall p l l',
+    contains_edge p l l' ->
+    exists p1 p2, p = p1++(l'::l::p2) /\ not (contains_edge p1 l l').
+Proof.
+  induction p as [p IHp] using (induction_ltof1 _ (fun x => length x)); unfold ltof in IHp.
+  intros l l' [p1 [p2 H]].
+  destruct (contains_edge_dec p2 l l').
+  + apply IHp in H0.
+    destruct H0 as [p3 [p4 [H01 H02]]].
+    subst. exists p3 , (p4 ++ l' :: l :: p1) ; split; eauto.
+    repeat rewrite app_comm_cons || rewrite app_assoc => //.
+    subst. rewrite app_length; simpl. Psatz.lia.
+  + exists p2, p1; split; eauto.
+Qed.
 
-  Lemma reachable_path_assignment :
-    forall σ σ' C ω ω' p f l l',
-      (getObj σ l) = Some (C, ω) ->
-      ω' = [f ↦ l']ω ->
-      σ' = [l ↦ (C, ω')]σ ->
-      reachable_path σ' p ->
-      contains_edge p l l' \/ reachable_path σ p.
-  Proof.
-    intros.
-    destruct (contains_edge_dec p l l') as [Hedge | Hedge]; eauto.
-    right.
-    induction p; eauto.
-    simpl in *.
-    destruct_match; [steps ; unfold dom in *; rewrite_anywhere update_one3 => // |].
-    subst. destructs. intuition auto.
-    + clear H2. clear H1. unfold reachable_one_step in *; steps.
-      destruct (PeanoNat.Nat.eq_dec l n); steps.
-      ++ rewrite_anywhere getObj_update1; eauto using getObj_dom.
-         invert_constructor_equalities; steps.
-         repeat eexists || eassumption. unfold getVal in *.
-         destruct (PeanoNat.Nat.eq_dec f f0); steps.
-         +++ rewrite_anywhere update_one1 ; eauto using nth_error_Some.
-             invert_constructor_equalities; steps.
-             exfalso; apply Hedge.
-             unfold contains_edge. exists l0, []; steps.
-             erewrite <- update_one3.
-             eapply nth_error_Some.
-             erewrite H0 => //.
-         +++ rewrite_anywhere update_one2; eauto .
-         +++ unfold dom in *. erewrite_anywhere update_one3; eauto.
-      ++ rewrite_anywhere getObj_update2; eauto using getObj_dom.
-         repeat eexists || eassumption.
-         unfold dom in *. erewrite <- update_one3; eauto.
-    + apply H2; clear H2.
-      unfold reachable_one_step, contains_edge in *.
-      intros. destructs.
-      apply Hedge. exists p1, (a::p2). rewrite H2.
-      rewrite app_comm_cons => //.
-  Qed.
-
-
-  Lemma reachability_first_step:
-    forall σ l1 l2,
-      σ ⊨ l1 ⇝ l2 ->
-      l1 = l2 \/ exists l0, reachable_one_step σ l1 l0.
-  Proof.
-    unfold reachable_one_step.
-    intros.
-    induction H; steps.
-    right.  repeat eexists; eauto.
-  Qed.
+Lemma reachable_path_assignment :
+  forall σ σ' C ω ω' p f l l',
+    (getObj σ l) = Some (C, ω) ->
+    ω' = [f ↦ l']ω ->
+    σ' = [l ↦ (C, ω')]σ ->
+    reachable_path σ' p ->
+    contains_edge p l l' \/ reachable_path σ p.
+Proof.
+  intros.
+  destruct (contains_edge_dec p l l') as [Hedge | Hedge]; eauto.
+  right.
+  induction p; eauto.
+  simpl in *.
+  destruct_match; [steps ; unfold dom in *; rewrite_anywhere update_one3 => // |].
+  subst. destructs. intuition auto.
+  + clear H2. clear H1. unfold reachable_one_step in *; steps.
+    destruct (PeanoNat.Nat.eq_dec l n); steps.
+    ++ rewrite_anywhere getObj_update1; eauto using getObj_dom.
+       invert_constructor_equalities; steps.
+       repeat eexists || eassumption. unfold getVal in *.
+       destruct (PeanoNat.Nat.eq_dec f f0); steps.
+       +++ rewrite_anywhere update_one1 ; eauto using nth_error_Some.
+           invert_constructor_equalities; steps.
+           exfalso; apply Hedge.
+           unfold contains_edge. exists l0, []; steps.
+           erewrite <- update_one3.
+           eapply nth_error_Some.
+           erewrite H0 => //.
+       +++ rewrite_anywhere update_one2; eauto .
+       +++ unfold dom in *. erewrite_anywhere update_one3; eauto.
+    ++ rewrite_anywhere getObj_update2; eauto using getObj_dom.
+       repeat eexists || eassumption.
+       unfold dom in *. erewrite <- update_one3; eauto.
+  + apply H2; clear H2.
+    unfold reachable_one_step, contains_edge in *.
+    intros. destructs.
+    apply Hedge. exists p1, (a::p2). rewrite H2.
+    rewrite app_comm_cons => //.
+Qed.
 
 
-  Lemma reachability_not_empty:
-    forall σ C l, l < dom σ -> (σ++[(C, [])]) ⊨ (length σ) ⇝ l -> False .
-  Proof.
-    intros.
-    apply reachability_first_step in H0; unfold dom in *; steps; try lia.
-    unfold reachable_one_step in *; steps.
-    rewrite_anywhere getObj_last; invert_constructor_equalities; destruct f; steps.
-  Qed.
-
-  Lemma reachability_ind2:
-    forall σ (P: Loc -> Loc -> Prop),
-      (forall l, P l l) ->
-      (forall l0 l1 C f ω, l1 < dom σ -> getObj σ l0 = Some (C, ω) -> getVal ω f = Some l1 -> P l0 l1) ->
-      (forall l0 l1 l2, σ ⊨ l0 ⇝ l1 -> P l0 l1 -> σ ⊨ l1 ⇝ l2 -> P l1 l2 -> P l0 l2) ->
-      forall l0 l1, σ ⊨ l0 ⇝ l1 -> P l0 l1.
-  Proof.
-    intros.
-    induction H2; eauto.
-  Qed.
+Lemma reachability_first_step:
+  forall σ l1 l2,
+    σ ⊨ l1 ⇝ l2 ->
+    l1 = l2 \/ exists l0, reachable_one_step σ l1 l0.
+Proof.
+  unfold reachable_one_step.
+  intros.
+  induction H; steps.
+  right.  repeat eexists; eauto.
+Qed.
 
 
+Lemma reachability_not_empty:
+  forall σ C l, l < dom σ -> (σ++[(C, [])]) ⊨ (length σ) ⇝ l -> False .
+Proof.
+  intros.
+  apply reachability_first_step in H0; unfold dom in *; steps; try lia.
+  unfold reachable_one_step in *; steps.
+  rewrite_anywhere getObj_last; invert_constructor_equalities; destruct f; steps.
+Qed.
 
-  Lemma reachability_empty:
-    forall σ C L l, l < dom σ -> ((σ++[(C, [])]) ⊫ L ⇝ l) -> (σ ⊫ L ⇝ l).
-  Proof.
-    intros.
-    inversion H0 as [l1 [Hl1 Hrch]].
-    exists l1; split => //.
-    apply reachable_path_reachability in Hrch as [Hrch | [p Hrch]].
-    + steps; eauto with rch.
-    + clear Hl1 H0. generalize dependent l. generalize dependent l1.
-      induction p; intros.
-      ++ steps; unfold reachable_one_step in *; steps.
-         repeat rewrite_anywhere dom_app.
-         eapply getObj_last_empty in H2; eauto; steps.
-         eapply rch_trans with l1; eauto using getObj_dom with rch.
-      ++ move: (app_cons_not_nil p nil l1) => Hp.
-         simpl in Hrch. destruct (p ++ [l1]) eqn:P; [exfalso; eauto |]. light.
-         unfold reachable_one_step in H0.
-         move: H0 => [C' [ω' [Hobja [[f Hval] Hdom]]]].
-         pose proof (getObj_last_empty _ _ _ _ _ _ _ Hobja Hval) as [Hobj Hl1].
-         light. eauto with rch.
-  Qed.
+Lemma reachability_ind2:
+  forall σ (P: Loc -> Loc -> Prop),
+    (forall l, P l l) ->
+    (forall l0 l1 C f ω, l1 < dom σ -> getObj σ l0 = Some (C, ω) -> getVal ω f = Some l1 -> P l0 l1) ->
+    (forall l0 l1 l2, σ ⊨ l0 ⇝ l1 -> P l0 l1 -> σ ⊨ l1 ⇝ l2 -> P l1 l2 -> P l0 l2) ->
+    forall l0 l1, σ ⊨ l0 ⇝ l1 -> P l0 l1.
+Proof.
+  intros.
+  induction H2; eauto.
+Qed.
 
 
-End Reachability.
+
+Lemma reachability_empty:
+  forall σ C L l, l < dom σ -> ((σ++[(C, [])]) ⊫ L ⇝ l) -> (σ ⊫ L ⇝ l).
+Proof.
+  intros.
+  inversion H0 as [l1 [Hl1 Hrch]].
+  exists l1; split => //.
+  apply reachable_path_reachability in Hrch as [Hrch | [p Hrch]].
+  + steps; eauto with rch.
+  + clear Hl1 H0. generalize dependent l. generalize dependent l1.
+    induction p; intros.
+    ++ steps; unfold reachable_one_step in *; steps.
+       repeat rewrite_anywhere dom_app.
+       eapply getObj_last_empty in H2; eauto; steps.
+       eapply rch_trans with l1; eauto using getObj_dom with rch.
+    ++ move: (app_cons_not_nil p nil l1) => Hp.
+       simpl in Hrch. destruct (p ++ [l1]) eqn:P; [exfalso; eauto |]. light.
+       unfold reachable_one_step in H0.
+       move: H0 => [C' [ω' [Hobja [[f Hval] Hdom]]]].
+       pose proof (getObj_last_empty _ _ _ _ _ _ _ Hobja Hval) as [Hobj Hl1].
+       light. eauto with rch.
+Qed.
