Wellformedness.v
@@ -1,299 +1,279 @@
-From Celsius Require Export Trees.
-From Celsius Require Export Eval.
-From Celsius Require Export PartialMonotonicity.
-From Celsius Require Export Reachability.
-From Celsius Require Export Compatibility.
-Require Import ssreflect ssrbool.
-Require Import Psatz.
-Require Import List.
+From Celsius Require Export Trees Eval PartialMonotonicity Reachability Compatibility.
+Require Import ssreflect ssrbool Psatz List.
 Import ListNotations.
 Open Scope nat_scope.
 Require Import Sets.Ensembles.
 
-(*
-  Notation "σ ⊨ l1 ⇝ l2" := (σ + l1 + l2) (at level 80, l1 at level 80, l2 at level 80).
-  Notation "σ1 ⇝ σ2 ⋖ L" := (σ1 * σ2 * L) (at level 81, σ2 at level 81).
-  Eval compute in (2 ⊨ 2 ⇝ 3) + (1 ⇝ 2 ⋖ 3).
-  Check (1 ⊨ 2 ⇝ 3).
-  Check (2 ⇝ 3 ⋖ 4).
- *)
+Create HintDb wf.
 
-Module Wellformedness.
-  Import Eval.Evaluator.
-  Import Reachability.
-  Create HintDb wf.
+Definition wf σ := forall l C ω, getObj σ l = Some(C,ω) -> forall f l, getVal ω f = Some l -> l < dom σ.
 
-  Definition wf σ := forall l C ω, getObj σ l = Some(C,ω) -> forall f l, getVal ω f = Some l -> l < dom σ.
-
-  Definition storeSubset (σ: Store) L := (forall l, (l ∈ L) -> l < (dom σ)).
-  Notation "L ⪽ σ" := (storeSubset σ L) (at level 80).
-  Definition codom (ρ: Env) : (LocSet):=
-    fun (l: Loc) => (List.In l ρ).
+Definition storeSubset (σ: Store) L := (forall l, (l ∈ L) -> l < (dom σ)).
+Notation "L ⪽ σ" := (storeSubset σ L) (at level 80).
+Definition codom (ρ: Env) : (LocSet):=
+  fun (l: Loc) => (List.In l ρ).
 
 
 
-  Lemma storeSubset_trans : forall a s s', dom s <= dom s' -> a ⪽ s -> a ⪽ s'.
-  Proof.
-    intros. intros l Hl.
-    pose proof (H0 l Hl).
-    lia.
-  Qed.
-  Hint Resolve storeSubset_trans: wf.
+Lemma storeSubset_trans : forall a s s', dom s <= dom s' -> a ⪽ s -> a ⪽ s'.
+Proof.
+  intros. intros l Hl.
+  pose proof (H0 l Hl).
+  lia.
+Qed.
+Hint Resolve storeSubset_trans: wf.
 
-  Lemma storeSubset_union : forall a b s, a ⪽ s -> b ⪽ s -> (a∪b) ⪽ s.
-  Proof.
-    unfold storeSubset; intros.
-    induction H1; eauto.
-  Qed.
-  Hint Resolve storeSubset_union: wf.
+Lemma storeSubset_union : forall a b s, a ⪽ s -> b ⪽ s -> (a∪b) ⪽ s.
+Proof.
+  unfold storeSubset; intros.
+  induction H1; eauto.
+Qed.
+Hint Resolve storeSubset_union: wf.
 
-  Lemma storeSubset_union_l : forall a b s, (a∪b) ⪽ s -> a ⪽ s.
-  Proof.
-    unfold storeSubset; intros.
-    apply H. eauto using Union_introl.
-  Qed.
-  Hint Resolve storeSubset_union_l: wf.
+Lemma storeSubset_union_l : forall a b s, (a∪b) ⪽ s -> a ⪽ s.
+Proof.
+  unfold storeSubset; intros.
+  apply H. eauto using Union_introl.
+Qed.
+Hint Resolve storeSubset_union_l: wf.
 
-  Lemma storeSubset_union_r : forall a b s, (a∪b) ⪽ s -> b ⪽ s.
-  Proof.
-    unfold storeSubset; intros.
-    apply H. eauto using Union_intror.
-  Qed.
-  Hint Resolve storeSubset_union_r: wf.
+Lemma storeSubset_union_r : forall a b s, (a∪b) ⪽ s -> b ⪽ s.
+Proof.
+  unfold storeSubset; intros.
+  apply H. eauto using Union_intror.
+Qed.
+Hint Resolve storeSubset_union_r: wf.
 
-  Lemma storeSubset_add : forall v a s,
-      codom (v :: a) ⪽ s <-> v < dom s /\ codom a ⪽ s.
-  Proof.
-    split; intros.
-    + unfold storeSubset in H.
-      split. apply H.
-      unfold codom, List.In, In; left => //.
-      intros l Hl. apply H.
-      unfold codom, List.In, In; right => //.
-    + intros l Hl. unfold codom, List.In, In in Hl. move: Hl=> [Hl|Hl]; steps.
-  Qed.
-  Hint Resolve storeSubset_add: wf.
+Lemma storeSubset_add : forall v a s,
+    codom (v :: a) ⪽ s <-> v < dom s /\ codom a ⪽ s.
+Proof.
+  split; intros.
+  + unfold storeSubset in H.
+    split. apply H.
+    unfold codom, List.In, In; left => //.
+    intros l Hl. apply H.
+    unfold codom, List.In, In; right => //.
+  + intros l Hl. unfold codom, List.In, In in Hl. move: Hl=> [Hl|Hl]; steps.
+Qed.
+Hint Resolve storeSubset_add: wf.
 
-  Notation " a ∪ { b } " := (Union Loc a (Singleton Loc b)) (at level 80).
-  Lemma storeSubset_singleton : forall a b σ, a ∪ {b} ⪽ σ -> b < dom σ.
-  Proof.
-    intros. apply (H b).
-    eauto using Union_intror, In_singleton.
-  Qed.
-  Hint Resolve storeSubset_singleton: wf.
+Notation " a ∪ { b } " := (Union Loc a (Singleton Loc b)) (at level 80).
+Lemma storeSubset_singleton : forall a b σ, a ∪ {b} ⪽ σ -> b < dom σ.
+Proof.
+  intros. apply (H b).
+  eauto using Union_intror, In_singleton.
+Qed.
+Hint Resolve storeSubset_singleton: wf.
 
-  Lemma storeSubset_singleton2 : forall a σ, (Singleton Loc a) ⪽ σ <-> a < dom σ.
-  Proof.
-    unfold storeSubset; steps;
+Lemma storeSubset_singleton2 : forall a σ, (Singleton Loc a) ⪽ σ <-> a < dom σ.
+Proof.
+  unfold storeSubset; steps;
     [induction (H a) | induction H0] ; steps.
-  Qed.
-  Hint Resolve storeSubset_singleton2: wf.
+Qed.
+Hint Resolve storeSubset_singleton2: wf.
 
-  Lemma storeSubset_codom_empty : forall s, codom [] ⪽ s.
-  Proof.
-    intros s l Hl.
-    steps.
-  Qed.
-  Hint Resolve storeSubset_codom_empty: wf.
+Lemma storeSubset_codom_empty : forall s, codom [] ⪽ s.
+Proof.
+  intros s l Hl.
+  steps.
+Qed.
+Hint Resolve storeSubset_codom_empty: wf.
 
-  Lemma codom_empty_union: forall a, (codom [] ∪ a) = a.
-  Proof.
-    intros.
-    apply Extensionality_Ensembles.
-    unfold Same_set. unfold Included; repeat steps || destruct H.
-    eapply Union_intror => //.
-  Qed.
-
-
-  Lemma wf_add : forall s c ρ, wf s -> codom ρ ⪽ s -> wf (s ++ [(c,ρ)]).
-  Proof.
-    unfold wf, dom; intros.
-    pose proof (getObj_dom _ _ _ H1).
-    pose proof (PeanoNat.Nat.eq_dec l (length s)) as [Hl0 | Hl0].
-    + rewrite app_length. simpl. subst.
-      rewrite getObj_last in H1. invert_constructor_equalities; subst.
-      rewrite PeanoNat.Nat.add_1_r. apply (PeanoNat.Nat.lt_trans _ (length s) _); try lia.
-      apply H0.
-      unfold getVal in H2. apply nth_error_In in H2. eauto.
-    + unfold dom in *. rewrite_anywhere app_length. simpl in H2.
-      rewrite PeanoNat.Nat.add_1_r in H3.
-      apply (PeanoNat.Nat.lt_succ_r l (length s)) in H3.
-      assert (l < length s) by lia.
-      rewrite app_length. simpl. unfold getObj in *.
-      rewrite nth_error_app1 in H1 => //.
-      apply (H _ _ _ H1) in H2. lia.
-  Qed.
-  Hint Resolve wf_add: wf.
-
-  Lemma wf_add_empty : forall s c, wf s -> wf (s ++ [(c,[])]).
-  Proof.
-    eauto using wf_add, storeSubset_codom_empty.
-  Qed.
-  Hint Resolve wf_add_empty: wf.
+Lemma codom_empty_union: forall a, (codom [] ∪ a) = a.
+Proof.
+  intros.
+  apply Extensionality_Ensembles.
+  unfold Same_set. unfold Included; repeat steps || destruct H.
+  eapply Union_intror => //.
+Qed.
 
 
-  Lemma wf_assign: forall σ σ' ω ω' l v f C,
-      (getObj σ l) = Some (C, ω) ->
-      σ' = [l ↦ (C, ω')]σ ->
-      ω' = [f ↦ v]ω ->
-      v < dom σ ->
-      wf σ -> wf σ'.
-  Proof.
-    unfold wf; steps. rewrite update_dom.
-    pose proof (PeanoNat.Nat.eq_dec l l0) as [Hl0 | Hl0]; subst.
-    + rewrite getObj_update1 in H4; eauto using getObj_dom.
-      unfold getVal in *.
-      assert (f0 < length ω0). {
-        pose proof (nth_error_Some ω0 f0);
+Lemma wf_add : forall s c ρ, wf s -> codom ρ ⪽ s -> wf (s ++ [(c,ρ)]).
+Proof.
+  unfold wf, dom; intros.
+  pose proof (getObj_dom _ _ _ H1).
+  pose proof (PeanoNat.Nat.eq_dec l (length s)) as [Hl0 | Hl0].
+  + rewrite app_length. simpl. subst.
+    rewrite getObj_last in H1. invert_constructor_equalities; subst.
+    rewrite PeanoNat.Nat.add_1_r. apply (PeanoNat.Nat.lt_trans _ (length s) _); try lia.
+    apply H0.
+    unfold getVal in H2. apply nth_error_In in H2. eauto.
+  + unfold dom in *. rewrite_anywhere app_length. simpl in H2.
+    rewrite PeanoNat.Nat.add_1_r in H3.
+    apply (PeanoNat.Nat.lt_succ_r l (length s)) in H3.
+    assert (l < length s) by lia.
+    rewrite app_length. simpl. unfold getObj in *.
+    rewrite nth_error_app1 in H1 => //.
+    apply (H _ _ _ H1) in H2. lia.
+Qed.
+Hint Resolve wf_add: wf.
+
+Lemma wf_add_empty : forall s c, wf s -> wf (s ++ [(c,[])]).
+Proof.
+  eauto using wf_add, storeSubset_codom_empty.
+Qed.
+Hint Resolve wf_add_empty: wf.
+
+
+Lemma wf_assign: forall σ σ' ω ω' l v f C,
+    (getObj σ l) = Some (C, ω) ->
+    σ' = [l ↦ (C, ω')]σ ->
+    ω' = [f ↦ v]ω ->
+    v < dom σ ->
+    wf σ -> wf σ'.
+Proof.
+  unfold wf; steps. rewrite update_dom.
+  pose proof (PeanoNat.Nat.eq_dec l l0) as [Hl0 | Hl0]; subst.
+  + rewrite getObj_update1 in H4; eauto using getObj_dom.
+    unfold getVal in *.
+    assert (f0 < length ω0). {
+      pose proof (nth_error_Some ω0 f0);
         destruct (nth_error ω0 f0); eapply_any; steps.
-      }
-      invert_constructor_equalities; subst.
-      pose proof (PeanoNat.Nat.eq_dec f f0) as [Hf | Hf]; subst.
-      ++ rewrite_anywhere update_one3.
-         rewrite update_one1 in H5 => // .
-         invert_constructor_equalities; steps.
-      ++ erewrite update_one2 in H5; eauto.
-    + unfold getObj in *.
-      rewrite update_one2 in H4; eauto using PeanoNat.Nat.neq_sym.
-  Qed.
-  Hint Resolve wf_assign: wf.
+    }
+    invert_constructor_equalities; subst.
+    pose proof (PeanoNat.Nat.eq_dec f f0) as [Hf | Hf]; subst.
+    ++ rewrite_anywhere update_one3.
+       rewrite update_one1 in H5 => // .
+       invert_constructor_equalities; steps.
+    ++ erewrite update_one2 in H5; eauto.
+  + unfold getObj in *.
+    rewrite update_one2 in H4; eauto using PeanoNat.Nat.neq_sym.
+Qed.
+Hint Resolve wf_assign: wf.
 
 
 
-  Theorem wellformedness_theorem_list_aux : forall k n ρ ψ,
-      (forall k : nat,
-          k < n ->
-          forall (e : Expr) (σ σ' : Store) (ρ : Env) (ψ l : Value),
-            (⟦ e ⟧ (σ, ρ, ψ )( k)) = Success l σ' -> wf σ -> (codom ρ ∪ {ψ}) ⪽ σ -> wf σ' /\ l < dom σ') ->
-      k < n ->
-      forall el s s' vl1 vl2,
-        fold_left (eval_list_aux ρ ψ k) el (Success_l vl1 s) = Success_l vl2 s' ->
-        wf s ->
-        codom vl1 ⪽ s ->
-        (codom ρ ∪ {ψ}) ⪽ s ->
-        wf s' /\ (codom vl2 ⪽ s') /\ (dom s <= dom s').
-  Proof.
-    intros k n ρ ψ H_strong Hn.
-    induction el; simpl; intros; try solve [steps].
-    destruct k => //; try solve [rewrite foldLeft_constant in H => //].
-    simpl in H.
-    destruct_eval.
+Theorem wellformedness_theorem_list_aux : forall k n ρ ψ,
+    (forall k : nat,
+        k < n ->
+        forall (e : Expr) (σ σ' : Store) (ρ : Env) (ψ l : Value),
+          (⟦ e ⟧ (σ, ρ, ψ )( k)) = Success l σ' -> wf σ -> (codom ρ ∪ {ψ}) ⪽ σ -> wf σ' /\ l < dom σ') ->
+    k < n ->
+    forall el s s' vl1 vl2,
+      fold_left (eval_list_aux ρ ψ k) el (Success_l vl1 s) = Success_l vl2 s' ->
+      wf s ->
+      codom vl1 ⪽ s ->
+      (codom ρ ∪ {ψ}) ⪽ s ->
+      wf s' /\ (codom vl2 ⪽ s') /\ (dom s <= dom s').
+Proof.
+  intros k n ρ ψ H_strong Hn.
+  induction el; simpl; intros; try solve [steps].
+  destruct k => //; try solve [rewrite foldLeft_constant in H => //].
+  simpl in H.
+  destruct_eval.
+  apply PeanoNat.Nat.lt_succ_l in Hn.
+  pose proof (H_strong k Hn _ _ _ _ _ _ H3 H0 H2) as [Hwfs2 Hv0].
+  pose proof (PartialMonotonicity.partialMonotonicity_theorem_dom _ _ _ _ _ _ _ H3).
+  assert (codom (v :: vl1) ⪽ s0) by (apply storeSubset_add; eauto using storeSubset_trans).
+  move /(_ _ _ _ _ H Hwfs2 H5 (storeSubset_trans _ s s0 H4 H2)): IHel => IHel.
+  steps; try lia.
+Qed.
+
+
+Theorem wellformedness_conserved :
+  forall k e σ σ' ρ ψ l,
+    ⟦e⟧(σ, ρ, ψ)(k) = (Success l σ') ->
+    wf σ ->
+    (codom ρ) ∪ {ψ} ⪽ σ ->
+    (wf σ' /\ l < dom σ').
+Proof.
+  apply (strong_induction (fun k => forall e σ σ' ρ ψ l, ⟦e⟧(σ, ρ, ψ)(k) = (Success l σ') -> wf σ -> (codom ρ) ∪ {ψ} ⪽ σ ->  (wf σ' /\ l < dom σ'))). intros.
+  assert (ψ < dom σ /\ forall l', List.In l' ρ -> l' < dom σ). {
+    unfold storeSubset in *.
+    split; steps; eauto using Union_introl, Union_intror, In_singleton. }
+  destruct_and.
+  destruct n => //.
+  move : (PeanoNat.Nat.lt_succ_diag_r n) => Hn.
+  destruct e ; simpl in H0 ;
+    repeat discriminate || subst || invert_constructor_equalities || destruct_match ||
+           lazymatch goal with
+           | H1 : ⟦ _ ⟧ ( _, _, _)( _ ) = Success _ _ |- _ =>
+             pose proof (PartialMonotonicity.partialMonotonicity_theorem_dom _ _ _ _ _ _ _ H1);
+               pose proof (H n Hn _ _ _ _ _ _ H1); clear H1 end; eauto.
+
+
+  + intuition auto. eauto using nth_error_In.
+  + intuition auto. unfold wf in *. eapply H6; eauto.
+  + destruct n => //. simpl in *.
     apply PeanoNat.Nat.lt_succ_l in Hn.
-    pose proof (H_strong k Hn _ _ _ _ _ _ H3 H0 H2) as [Hwfs2 Hv0].
-    pose proof (PartialMonotonicity.partialMonotonicity_theorem_dom _ _ _ _ _ _ _ H3).
-    assert (codom (v :: vl1) ⪽ s0) by (apply storeSubset_add; eauto using storeSubset_trans).
-    move /(_ _ _ _ _ H Hwfs2 H5 (storeSubset_trans _ s s0 H4 H2)): IHel => IHel.
-    steps; try lia.
-  Qed.
+    pose proof (wellformedness_theorem_list_aux n (S(S n)) ρ ψ H Hn _ _ _ _ _ matched3) as H_list.
+    assert (codom [] ⪽ s) by done.
+    assert ((codom ρ ∪ {ψ}) ⪽ s) by eauto using storeSubset_trans.
+    apply H6; intuition auto.
+    intros l2 Hl2; induction Hl2; eauto.
+    induction H6. lia.
+  + destruct n => //. simpl in *.
+    apply PeanoNat.Nat.lt_succ_l in Hn.
+    pose proof (wellformedness_theorem_list_aux n (S(S n)) ρ ψ H Hn _ _ _ _ _ matched H1 (storeSubset_codom_empty _) H2) as [H_wf_s [H_codom_s H_dom_s]].
+    repeat destruct_match; try discriminate.
+    assert (forall k fields l σ1 σ2,
+               k < S (S n) ->
+               fold_left (init_field l1 l k) fields (Some σ1) = Some σ2 ->
+               (codom l1 ∪ {l}) ⪽ σ1 ->
+               wf σ1 ->
+               wf σ2 /\ (dom σ1 <= dom σ2)). {
+      induction fields0; simpl; intros; try solve [steps].
+      destruct k; simpl in H5; try solve [rewrite_anywhere foldLeft_constant  => //].
+      destruct a.
+      destruct_eval.
+      unfold assign_new in *. destruct_match; try solve [rewrite_anywhere foldLeft_constant  => //].
+      destruct o.
+      pose proof (PartialMonotonicity.partialMonotonicity_theorem_dom _ _ _ _ _ _ _ H8).
+      apply H in H8 => // ; try lia. destruct H8 as [E1 E2].
+      apply IHfields0 in H5; clear IHfields0 => //.
+      ++ steps. unfold dom in *; rewrite_anywhere update_one3. eauto using PeanoNat.Nat.le_trans.
+      ++ apply (storeSubset_trans _ σ1 s0) in H6 => //.
+         apply (storeSubset_trans _ s0) => //.
+         unfold dom in *.
+         rewrite update_one3; eauto.
+      ++ clear H5.
+         intros l'; intros.
+         unfold dom in *. rewrite update_one3.
+         move: (PeanoNat.Nat.eq_dec l l') => [Hl' | Hl'].
+         +++ (* l = l' *)
+           subst.
+           rewrite getObj_update1 in H5; eauto using getObj_dom. invert_constructor_equalities; subst.
+           unfold getVal in *. apply nth_error_Some2 in H8. destruct H8 as [H8 | H8]; subst; eauto.
+         +++ (* l ≠ l' *)
+           unfold getObj in *.
+           rewrite update_one2 in H5 => //. eapply E1; eauto.
+    }
+    apply H0 in matched0; eauto using wf_add_empty.
+    split; steps.
+    unfold dom in *; rewrite_anywhere app_length. simpl in *. lia.
+    apply storeSubset_union. apply (storeSubset_trans _ s _) => //. unfold dom in *; rewrite app_length; lia.
+    unfold storeSubset; intros. induction H5. unfold dom in *; rewrite app_length; simpl ; lia.
+  + unfold assign in *.
+    destruct (getObj s0 v0) eqn:G.
+    ++ destruct o.
+       apply H6. intuition auto.
+       eapply wf_assign; eauto; try eapply H9; eauto using storeSubset_trans.
+       apply (storeSubset_trans _ σ _) => //.
+       unfold dom in *; rewrite update_one3. lia.
+    ++ repeat apply_any; eauto using storeSubset_trans.
+Qed.
+Hint Resolve wellformedness_conserved: wf.
 
 
-  Theorem wellformedness_conserved :
-    forall k e σ σ' ρ ψ l,
-      ⟦e⟧(σ, ρ, ψ)(k) = (Success l σ') ->
-      wf σ ->
-      (codom ρ) ∪ {ψ} ⪽ σ ->
-      (wf σ' /\ l < dom σ').
-  Proof.
-    apply (strong_induction (fun k => forall e σ σ' ρ ψ l, ⟦e⟧(σ, ρ, ψ)(k) = (Success l σ') -> wf σ -> (codom ρ) ∪ {ψ} ⪽ σ ->  (wf σ' /\ l < dom σ'))). intros.
-    assert (ψ < dom σ /\ forall l', List.In l' ρ -> l' < dom σ). {
-      unfold storeSubset in *.
-      split; steps; eauto using Union_introl, Union_intror, In_singleton. }
-    destruct_and.
-    destruct n => //.
-    move : (PeanoNat.Nat.lt_succ_diag_r n) => Hn.
-    destruct e ; simpl in H0 ;
-      repeat discriminate || subst || invert_constructor_equalities || destruct_match ||
-             lazymatch goal with
-             | H1 : ⟦ _ ⟧ ( _, _, _)( _ ) = Success _ _ |- _ =>
-               pose proof (PartialMonotonicity.partialMonotonicity_theorem_dom _ _ _ _ _ _ _ H1);
-                 pose proof (H n Hn _ _ _ _ _ _ H1); clear H1 end; eauto.
+Theorem wf_conserved :
+  forall k e σ σ' ρ ψ l,
+    ⟦e⟧(σ, ρ, ψ)(k) = (Success l σ') ->
+    wf σ ->
+    (codom ρ) ∪ {ψ} ⪽ σ ->
+    wf σ'.
+Proof.
+  intros. eapply wellformedness_conserved; eauto.
+Qed.
 
+Theorem correct_value :
+  forall k e σ σ' ρ ψ l,
+    ⟦e⟧(σ, ρ, ψ)(k) = (Success l σ') ->
+    wf σ ->
+    (codom ρ) ∪ {ψ} ⪽ σ ->
+    l < dom σ'.
+Proof.
+  intros. eapply wellformedness_conserved; eauto.
+Qed.
 
-    + intuition auto. eauto using nth_error_In.
-    + intuition auto. unfold wf in *. eapply H6; eauto.
-    + destruct n => //. simpl in *.
-      apply PeanoNat.Nat.lt_succ_l in Hn.
-      pose proof (wellformedness_theorem_list_aux n (S(S n)) ρ ψ H Hn _ _ _ _ _ matched3) as H_list.
-      assert (codom [] ⪽ s) by done.
-      assert ((codom ρ ∪ {ψ}) ⪽ s) by eauto using storeSubset_trans.
-      apply H6; intuition auto.
-      intros l2 Hl2; induction Hl2; eauto.
-      induction H6. lia.
-    + destruct n => //. simpl in *.
-      apply PeanoNat.Nat.lt_succ_l in Hn.
-      pose proof (wellformedness_theorem_list_aux n (S(S n)) ρ ψ H Hn _ _ _ _ _ matched H1 (storeSubset_codom_empty _) H2) as [H_wf_s [H_codom_s H_dom_s]].
-      repeat destruct_match; try discriminate.
-      assert (forall k fields l σ1 σ2,
-                 k < S (S n) ->
-                 fold_left (init_field l1 l k) fields (Some σ1) = Some σ2 ->
-                 (codom l1 ∪ {l}) ⪽ σ1 ->
-                 wf σ1 ->
-                 wf σ2 /\ (dom σ1 <= dom σ2)). {
-        induction fields0; simpl; intros; try solve [steps].
-        destruct k; simpl in H5; try solve [rewrite_anywhere foldLeft_constant  => //].
-        destruct a.
-        destruct_eval.
-        unfold assign_new in *. destruct_match; try solve [rewrite_anywhere foldLeft_constant  => //].
-        destruct o.
-        pose proof (PartialMonotonicity.partialMonotonicity_theorem_dom _ _ _ _ _ _ _ H8).
-        apply H in H8 => // ; try lia. destruct H8 as [E1 E2].
-        apply IHfields0 in H5; clear IHfields0 => //.
-        ++ steps. unfold dom in *; rewrite_anywhere update_one3. eauto using PeanoNat.Nat.le_trans.
-        ++ apply (storeSubset_trans _ σ1 s0) in H6 => //.
-           apply (storeSubset_trans _ s0) => //.
-           unfold dom in *.
-           rewrite update_one3; eauto.
-        ++ clear H5.
-           intros l'; intros.
-           unfold dom in *. rewrite update_one3.
-           move: (PeanoNat.Nat.eq_dec l l') => [Hl' | Hl'].
-           +++ (* l = l' *)
-             subst.
-             rewrite getObj_update1 in H5; eauto using getObj_dom. invert_constructor_equalities; subst.
-             unfold getVal in *. apply nth_error_Some2 in H8. destruct H8 as [H8 | H8]; subst; eauto.
-           +++ (* l ≠ l' *)
-             unfold getObj in *.
-             rewrite update_one2 in H5 => //. eapply E1; eauto.
-        }
-      apply H0 in matched0; eauto using wf_add_empty.
-      split; steps.
-      unfold dom in *; rewrite_anywhere app_length. simpl in *. lia.
-      apply storeSubset_union. apply (storeSubset_trans _ s _) => //. unfold dom in *; rewrite app_length; lia.
-      unfold storeSubset; intros. induction H5. unfold dom in *; rewrite app_length; simpl ; lia.
-    + unfold assign in *.
-      destruct (getObj s0 v0) eqn:G.
-      ++ destruct o.
-         apply H6. intuition auto.
-         eapply wf_assign; eauto; try eapply H9; eauto using storeSubset_trans.
-         apply (storeSubset_trans _ σ _) => //.
-         unfold dom in *; rewrite update_one3. lia.
-      ++ repeat apply_any; eauto using storeSubset_trans.
-  Qed.
-  Hint Resolve wellformedness_conserved: wf.
-
-
-  Theorem wf_conserved :
-    forall k e σ σ' ρ ψ l,
-      ⟦e⟧(σ, ρ, ψ)(k) = (Success l σ') ->
-      wf σ ->
-      (codom ρ) ∪ {ψ} ⪽ σ ->
-      wf σ'.
-  Proof.
-    intros. eapply wellformedness_conserved; eauto.
-  Qed.
-
-  Theorem correct_value :
-    forall k e σ σ' ρ ψ l,
-      ⟦e⟧(σ, ρ, ψ)(k) = (Success l σ') ->
-      wf σ ->
-      (codom ρ) ∪ {ψ} ⪽ σ ->
-      l < dom σ'.
-  Proof.
-    intros. eapply wellformedness_conserved; eauto.
-  Qed.
-
-  Hint Resolve wf_conserved: wf.
-  Hint Resolve correct_value: wf.
-
-
-End Wellformedness.
+Hint Resolve wf_conserved: wf.
+Hint Resolve correct_value: wf.
